src/Compiler.v
@@ -1,23 +1,23 @@
-Require Core Front RTL Flat CSE FirstOrder. 
+Require Core Front IR RTL CSE FirstOrder. 
 
 
-Definition Compile Phi t  (a : forall Var, Front.action Phi Var t) : Flat.Block Phi t :=
-  let x := RTL.Compile Phi  t a in
-  let x := Flat.Compile Phi t x in 
+Definition Compile Phi t  (a : forall Var, Front.action Phi Var t) : RTL.Block Phi t :=
+  let x := IR.Compile Phi  t a in
+  let x := RTL.Compile Phi t x in 
   let x := CSE.Compile Phi t  x in  
         x. 
 
 Lemma Compile_correct (Phi : Core.state) t a :
   let block := Compile Phi t a in 
-    Flat.WF Phi t (Flat.Compile _ _(RTL.Compile _ _ a)) -> 
+    RTL.WF Phi t (RTL.Compile _ _(IR.Compile _ _ a)) -> 
   forall st Delta, 
-    Flat.Eval Phi st t block Delta =
+    RTL.Eval Phi st t block Delta =
     Front.Eval Phi st t a Delta. 
 Proof.
   unfold Compile. intros. 
   rewrite CSE.Compile_correct. 
-  rewrite Flat.Compile_correct. 
   rewrite RTL.Compile_correct. 
+  rewrite IR.Compile_correct. 
   reflexivity. 
   apply H. 
 Qed. 
