src/RTL.v
@@ -1,348 +1,222 @@
-Require Import Common. 
-Require Import Core.   
-Require Import Front. 
-  
+Require Common Core Front IR Equality.
+
+Import Common. 
+
 Section t. 
-  Variable Phi : state. 
-  Notation updates := (DList.T (option ∘ eval_sync) Phi). 
+  Variable Phi : Core.state. 
+  
+  Notation updates := (DList.T (Common.comp option  Core.eval_sync) Phi). 
   
   Section defs. 
-  Variable R : type -> Type. 
-  (** Combinational bindings (expressions, register reads)  *)
-  Inductive bind (t : type) : Type := 
-  | bind_expr :  expr R t ->  bind t
-  | bind_reg_read : var Phi (Treg t) -> bind t
-  | bind_regfile_read : forall n, var Phi (Tregfile n t) -> R ( (Tint n)) -> bind t. 
+    Import Core. 
+    Variable Var : type -> Type. 
     
-  Inductive telescope (A : Type): Type :=
-  | telescope_end : A -> telescope A
-  | telescope_bind : forall arg, bind arg -> (R arg -> telescope A) -> telescope A. 
+    Inductive expr : type -> Type :=
+    | Evar : forall t, Var t -> expr t
+    | Eread : forall t,  var Phi (Treg t) -> expr t
+    | Eread_rf : forall n t, var Phi (Tregfile n t) -> Var (Tint n) -> expr t 
+    | Ebuiltin : forall (args : list type) (res : type),
+                   builtin args res ->
+                   DList.T Var args ->
+                   expr res
+    | Econstant : forall ty : type, constant ty -> expr ty
+    | Emux : forall t : type,
+               Var Tbool ->  Var t -> Var t -> expr  t
+    | Efst : forall (l : list type) (t : type),
+               Var (Ttuple (t :: l)) -> expr t
+    | Esnd : forall (l : list type) (t : type),
+               Var (Ttuple (t :: l)) -> expr (Ttuple l)
+    | Enth : forall (l : list type) (t : type),
+               var l t -> Var (Ttuple l) -> expr t
+    | Etuple : forall l : list type,
+                 DList.T (Var) l -> expr  (Ttuple l). 
+        
+    Inductive telescope (A : Type): Type :=
+    | telescope_end : A -> telescope A
+    | telescope_bind : forall arg, expr arg -> (Var arg -> telescope A) -> telescope A. 
+        
+    Fixpoint compose {A B}
+                     (tA : telescope  A)
+                     (f : A -> telescope  B) :
+      telescope  B :=
+      match tA with
+        | telescope_end e => f e
+        | telescope_bind arg b cont => telescope_bind _  arg b (fun x => compose (cont x) f)
+      end.
+    Notation "e :-- t1 ; t2 " := (compose t1 (fun e => t2)) (right associativity, at level 80, e1 at next level).
+      
+    Inductive effect  : sync -> Type :=
+    | effect_reg_write : forall t,  Var t -> Var Tbool -> effect (Treg t)
+    | effect_regfile_write : forall n t,  Var t -> Var (Tint n) -> Var Tbool -> 
+                                     effect (Tregfile n t). 
     
-  (* nested effects *)
-  Inductive neffect  : Type :=
-  | neffect_guard : forall (guard : expr R Tbool), list (neffect) -> neffect 
-  | neffect_reg_write : forall t, var Phi (Treg t) -> R t -> neffect
-  | neffect_regfile_write : forall n t, var Phi (Tregfile n t) -> R ( (Tint n)) -> R t -> neffect. 
-
-  Definition nblock t := telescope (R t * expr R Tbool * list neffect)%type. 
-  
-  Fixpoint compose {A B}
-                   (tA : telescope  A)
-                   (f : A -> telescope  B) :
-    telescope  B :=
-    match tA with
-      | telescope_end e => f e
-      | telescope_bind arg b cont => telescope_bind _  arg b (fun x => compose (cont x) f)
-    end.
-
-  Definition compose_block {t B} 
-                           (tA : nblock t)
-                           (f : R t -> expr R Tbool -> list neffect -> telescope B) :
-    telescope B :=
-    compose tA (fun x => match x with ((r,g),e) => f r g e end). 
-  Hint Unfold compose_block. 
-  Notation "x <- e1 ; e2" := (telescope_bind _ _ e1 (fun x => e2)) (right associativity, at level 80, e1 at next level).  
-  Notation " & e " := (telescope_end _ e) (at level 71). 
-  Notation "[< r , g , e >] :- t1 ; t2 " := (compose_block t1 (fun r g e => t2)) (right associativity, at level 80, t1 at next level). 
-  
-  Arguments neffect_guard guard%expr neffects%list. 
-  
-  (** * Compilation *)
-  (** This 'smart constructor' reduces the size of the guard, by using
-  the fact that [true] is a neutral element for [&&] *)
-  
-  Definition andb (a b : expr R Tbool): expr R Tbool :=
-    match a, b with 
-      | Econstant Tbool x, o 
-      | o, Econstant Tbool x => if x then o else (#b false)%expr
-      | _, _ => (a && b)%expr
-    end. 
-  
-
-  Definition orb (a b : expr R Tbool): expr R Tbool :=
-    match a, b with 
-      | Econstant Tbool x, o 
-      | o, Econstant Tbool x => if x then (#b true) else o
-      | _, _ => (a || b)%expr
-    end. 
-  
-  Definition convert  l : DList.T (expr R) l -> Tuple.of_list (expr R) l := 
-    DList.to_tuple (fun t X => X). 
-
-  Fixpoint map T F F' (G : forall t, F t -> F' t) (l : list T) : 
-    Tuple.of_list F l -> Tuple.of_list F' l:=
-    match l with 
-      | nil => fun x => x
-      | cons t q => fun x => (G t (fst x), map T F F' G q (snd x))
-    end. 
-
-  Arguments map {T F F'} G l _. 
-
-  (**  The compilation function itself *)  
-  Definition compile_inner (unit : R Tunit) t (a : action Phi R t) : telescope (R t * expr R Tbool * list neffect).  
-  refine (
-      let f := fix compile t (a : action Phi R t) : telescope (R t * expr R Tbool * list neffect):= 
-          match a with 
-            | Return t exp =>  
-                x <- (bind_expr _ exp); 
-                & (x, #b true, nil)
-            | Bind t u A F => 
-                [< rA, gA, eA >] :- compile _ A;
-                [< rB, gB, eB >] :- compile _ (F rA); 
-                & (rB, andb gA gB, List.app eA eB)             
-            | Assert exp => 
-                x <- (bind_expr _ exp); 
-                & (unit, !x, nil)%expr
-            | Primitive args res p exprs => _
-            (* | Try A =>  *)
-            (*     [< rA, gA, eA >] :- compile _ A; *)
-            (*     let e := neffect_guard gA eA in *)
-            (*       & (varunit, #b true, [e])%list *)
-            (*     (* & (varunit, gA, eA) *) *)
-            | OrElse t A A' => 
-                [< rA, gA, eA >] :- compile _ A;
-                [< rA', gA', eA' >] :- compile _ A';
-                let e := neffect_guard gA eA in 
-                let e' := neffect_guard (andb (~ gA)  gA')%expr eA' in 
-                  r <- (bind_expr _ (Emux _ _ gA (!rA) (!rA'))%expr); 
-                  & ( r , (orb gA gA')%expr , [e;e'])%list
-          end in f t a).
-  (* primitive *)
-  revert exprs. 
-  refine (match p with
-            | register_read t v => _
-            | register_write t v => _
-            | regfile_read n t v  => _
-            | regfile_write n t v  => _
-          end); clear p; intros exprs. 
-  (* register read *)
-  refine (x <- (bind_reg_read _ v); &(x, #b true, nil)). 
-  (* register write *)
-  refine ( let env := convert _ exprs in 
-             let w := fst env in 
-               x <- bind_expr _ w; 
-           let e := ([neffect_reg_write _ v x])%list  in 
-             &( unit, #b true, e)
-         ). 
-  (* register file read *)
-  refine ( let env := convert _ exprs in 
-             let adr := fst env in 
-               adr <- bind_expr _ adr; 
-           x <- bind_regfile_read _ _ v adr; 
-           &( x, #b true, nil)
-         ). 
-  (* register file write *)
-  refine ( let env := convert _ exprs in 
-             match env with 
-               | (adr, (w, _)) => 
-                   adr <- bind_expr _ adr; 
-                   w <- bind_expr _ w;
-                   let e :=  ([neffect_regfile_write _ _ v  adr w])%list in                      
-                     &( unit, #b true, e)                      
-             end
-         ). 
-    (* or else *)  
-  Defined. 
-    Definition compile t a :=   
-      (unit <- (bind_expr _ (# Ctt))%expr; compile_inner unit t a). 
-
-  
-  Inductive effect  : sync -> Type :=
-  | effect_reg_write : forall t,  R t -> R Tbool -> effect (Treg t)
-  | effect_regfile_write : forall n t,  R t -> R ( (Tint n)) -> R Tbool -> 
-                                                effect (Tregfile n t). 
-  
-  Definition effects := DList.T (option ∘ effect) Phi. 
-  
-  Definition init_effects : effects := DList.init sync (option ∘ effect) (fun t : sync => None) Phi. 
-
-  Definition block t := telescope (R t * expr R Tbool *  effects). 
+    Definition effects := DList.T (option ∘ effect) Phi. 
     
-  Notation "e :-- t1 ; t2 " := (compose t1 (fun e => t2)) (right associativity, at level 80, e1 at next level).
-  Arguments Tuple.set {T F l t} _ _ _.  
-
-  Definition nblock_to_block {t} (B : nblock t) : block t. 
-  unfold block, nblock in *. 
-  
-  Definition inversion_effect_Treg t (e : effect (Treg t)) : (R t * R Tbool) :=
-    match e with 
-      | effect_reg_write _ x y => (x,y)
-    end. 
-
-  Definition inversion_effect_Tregfile t n (e: effect (Tregfile n t)): 
-    (R t * R ( (Tint n)) *R Tbool) :=
-    match e with 
-      | effect_regfile_write _ _ x y z => (x,y,z)
-    end. 
-
-  Definition merge s (a b : effect s) : telescope (effect s). 
-  refine (match s as s'  return effect s' -> effect s' -> telescope (effect s') with 
-              | Treg t => fun a b => 
-                           let (va,ga) := inversion_effect_Treg t a in 
-                           let (vb,gb) := inversion_effect_Treg t b in 
-                             (
-                               we <- bind_expr  _ (!ga || !gb)%expr ;
-                               w <- bind_expr  _ (Emux _ _ (!ga) (!va) (!vb) )%expr ;
-                               & (effect_reg_write  _ w we))
-              | Tregfile n t => fun a b => 
-                           match inversion_effect_Tregfile t n a with 
-                             | (va,adra,ga) =>
-                                 match inversion_effect_Tregfile t n b with 
-                                   | (vb,adrb,gb) =>
-                                       (
-                                         we <- bind_expr  _ (orb (!ga) (!gb))%expr; 
-                                         wadr <- bind_expr _ (Emux _ _ (!ga) (!adra) (!adrb))%expr; 
-                                         wdata <- bind_expr _ (Emux _ _ (!ga) (!va) (!vb))%expr; 
-                                         &  (effect_regfile_write _ _ wdata wadr we))
-                                 end
-                           end
-          end a b). 
-  Defined. 
-
-    (** We give the priority to the old write here  *)
-  Definition update t (v : var Phi t) (e : effect t)  (acc: effects) : telescope effects. 
-  refine ( match DList.get  v acc with 
-               | Some old => 
-                   e :-- merge t old e ; & (DList.set v (Some e) acc)
-               | None => 
-                   & (DList.set v (Some e) acc)
-           end). 
-  Defined. 
-                                                                       
-
-  Fixpoint compile_neffect (G : expr R Tbool) (E : neffect) (B : effects) : telescope effects :=
-    match E with               
-      | neffect_guard guard L => 
-                    let compile_neffects := fix compile_neffects G l U :=
-                        match l with 
-                          | nil =>  & U
-                          | cons t q => 
-                              compose (compile_neffect G t U)
-                                      (compile_neffects G q)
-                        end in 
-                      compile_neffects (andb G  guard)%expr L B
-      | neffect_reg_write t v val => 
-          G <- bind_expr _  G;
-          update (Treg t) v (effect_reg_write t val G) B
-      | neffect_regfile_write n t v adr val => 
-          G <- bind_expr _  G;
-          update (Tregfile n t) v (effect_regfile_write n t val adr G) B
-    end.  
-
+    Definition block t := telescope (Var t * Var Tbool *  effects). 
+    Notation "x :- e1 ; e2" := (telescope_bind  _ _  e1 (fun x => e2)) (right associativity, at level 80, e1 at next level).  
+    Notation " & e " := (telescope_end _  e) (at level 71). 
     
-  Fixpoint compile_neffects (G : expr R Tbool)(l : list neffect)  (T : effects) :
-    telescope effects :=
-    match l with 
-      | nil =>  & T
-      | cons t q => 
-          compose (compile_neffect G  t T)
-                  (compile_neffects G q)
-    end. 
-
-  (* guard was replaced by true  *)
-  refine (compose_block B (fun res guard neffects => 
-                             compose (compile_neffects (guard ) neffects (init_effects))
-                             (fun effects => &(res, guard, effects)))). 
-  Defined. 
-
-
-  End defs. 
-  
-  (** * Semantics *)
-  Section sem. 
-    Variable st : eval_state Phi. 
-    Definition eval_bind t (b : bind eval_type t) : (eval_type t).
-    refine (match b with
-              | bind_expr x =>  (eval_expr _ x)
-              | bind_reg_read v => (DList.get v st)
-              | bind_regfile_read n v adr => 
-                  let rf := DList.get  v st in
-                    Regfile.get rf (adr)                
-            end
-           ). 
+    
+    Definition compile_expr t (e : Front.expr Var t) : telescope (Var t).
+    refine (
+        let fix fold t (e : Front.expr Var t) :=
+            let fix of_list (l : list type) (x : DList.T (Front.expr Var) l) : telescope (DList.T Var l) :=
+                match x in  (DList.T _ l)
+                   return
+                   (telescope (DList.T Var l)) with 
+                      | DList.nil => & ([])%dlist
+                      | DList.cons t q dt dq => 
+                          x  :-- fold t dt;
+                          dq :--   of_list q dq;   
+                          &  (x :: dq)%dlist
+                end in
+              
+              match e with
+                | Front.Evar t v => & v
+                | Front.Ebuiltin args res f x => 
+                    x :-- of_list args x; 
+                    y :- Ebuiltin args res f x; 
+                    &y 
+                | Front.Econstant ty c => c :- Econstant _ c; &c
+                | Front.Emux t c l r => 
+                    c :-- fold _ c;
+                    l :-- fold _ l;
+                    r :-- fold _ r;
+                    ret :- (Emux t c l r) ;
+                    & ret
+                | Front.Efst l t x => 
+                    x :-- fold _ x; ret :- Efst l t x; & ret
+                | Front.Esnd l t x => 
+                    x :-- fold _ x; ret :- Esnd l t x; & ret
+                | Front.Enth l t m x => 
+                    x :-- fold _ x; ret :- Enth l t m x; & ret
+                | Front.Etuple l exprs => 
+                    exprs :-- of_list l exprs; ret :- Etuple l exprs; &ret
+              end in fold t e).
     Defined. 
     
-                                                                
-    Fixpoint eval_neffect (e :neffect eval_type) (Delta : updates) : updates :=    
-      match e with 
-        | neffect_guard g l' => 
-            let fix eval_neffects l Delta := 
-                match l with 
-                  | nil => Delta
-                  | cons e q =>  
-                      let Delta := eval_neffect e Delta in 
-                        eval_neffects q Delta
-                end in     
-              match eval_expr _ g with 
-                | true => 
-                    eval_neffects l' Delta
-                | false => Delta
-            end
-      | neffect_reg_write t v w =>                                               
-          Front.Diff.add Phi Delta (Treg t) v w 
-      | neffect_regfile_write  n t v adr w  =>  
-          let rf := DList.get v st in                          
-            let rf := Regfile.set rf adr  w in 
-              Front.Diff.add Phi Delta (Tregfile n t) v rf            
-    end. 
-  
-    Fixpoint eval_neffects ( l : list (neffect eval_type)) Delta : updates :=
-      match l with 
-        | nil =>  Delta
-        | cons e q => (* do Delta <- eval_neffect e Delta;  *)
-            let Delta :=  (eval_neffect e Delta) in 
-            eval_neffects q Delta
+    Fixpoint compile_exprs l (x: DList.T (Front.expr Var) l) :  telescope (DList.T Var l) :=
+      match x in  (DList.T _ l)
+         return
+         (telescope (DList.T Var l)) with 
+        | DList.nil => & ([])%dlist
+        | DList.cons t q dt dq => 
+            x  :-- compile_expr t dt;
+            dq :--   compile_exprs q dq;   
+            &  (x :: dq)%dlist
       end. 
-  
-    Lemma fold_eval_neffects :
-      (fix eval_neffects l Delta := 
-       match l with 
-                | nil =>  Delta
-                | cons e q => 
-                    let Delta := (eval_neffect e Delta) in 
-                      (* do Delta <- eval_neffect e Delta;  *)
-                      eval_neffects q Delta
-       end)= eval_neffects .
-    Proof. 
-      unfold eval_neffects. reflexivity.
-    Qed. 
     
-    Fixpoint eval_nblock t  (T : nblock  eval_type t) :
-      updates -> option (eval_type t * updates) := 
-      match T with
-        | telescope_bind arg bind cont => 
-            fun Delta => 
-              let res := eval_bind _ bind in
-              eval_nblock _ (cont res) Delta
-        | telescope_end (p, g, e) => fun Delta =>
-                                      let g := eval_expr _ g  in             
-                                      if g then                                         
-                                        Some (p, eval_neffects e Delta)
-                                      else None
-    end. 
+    Lemma compile_exprs_fold : 
+      (fix of_list (l : list Core.type)
+           (x0 : Common.DList.T
+                       (Front.expr Var) l)
+           {struct x0} :
+       telescope 
+                   (Common.DList.T Var l) :=
+       match
+         x0 in (Common.DList.T _ l0)
+          return
+          (telescope (Common.DList.T Var l0))
+       with
+         | Common.DList.nil => & Common.DList.nil
+         | Common.DList.cons t1 q0 dt dq =>
+             x1 :-- compile_expr t1 dt;
+             dq0 :-- of_list q0 dq; & Common.DList.cons x1 dq0
+       end) = compile_exprs. 
+    Proof. reflexivity. Qed. 
     
+    Definition compile_effects (e : IR.effects Phi Var)  : effects. 
+    unfold effects. refine  (DList.map _  e).
+    intros a x.
+    refine (match x with
+              | None => None
+              | Some x => match x with 
+                           | IR.effect_reg_write t v g => 
+                               Some (effect_reg_write t v g)
+                           | IR.effect_regfile_write n t v adr g =>
+                               Some (effect_regfile_write n t v adr g)
+                         end
+            end).
     
-    Arguments Tuple.set {T F l t} v _ _. 
-    Definition eval_effects (e : effects eval_type) (Delta : updates) : updates.  
+    Defined. 
+    
+    Definition compile t  (b : IR.block Phi Var t) : block t.     
+    refine (let fold := fix fold t (b : IR.block Phi Var t) : block t :=
+                match b with 
+                  | IR.telescope_end x => 
+                      match x with 
+                          (r, g,e) => g :-- compile_expr _ g; & (r,g,compile_effects e)
+                        end
+                  | IR.telescope_bind a bd k => 
+                      match bd with
+                        | IR.bind_expr x => 
+                            x :-- compile_expr _ x ; fold _ (k x)
+                        | IR.bind_reg_read x => 
+                            x :- Eread a x; fold _ (k x)
+                        | IR.bind_regfile_read n x x0 => 
+                            x :- Eread_rf n a x x0; fold _ (k x)
+                      end
+                end in fold t b                         
+           ). 
+      Defined. 
+  End defs. 
+  Section sem. 
+    
+    Variable st : Core.eval_state Phi. 
+    
+    Definition eval_expr (t : Core.type) (e : expr Core.eval_type t) : Core.eval_type t. 
+    refine ( 
+        let fix eval_expr t (e : expr Core.eval_type t) {struct e} : Core.eval_type t:=
+            match e with
+              | Evar t v => v
+              | Eread t v => (Common.DList.get v st)
+              | Eread_rf n t v adr =>  
+                  let rf := Common.DList.get  v st in
+                    Common.Regfile.get rf (adr)                
+
+              | Ebuiltin args res f exprs => 
+                  let exprs := 
+                      Common.DList.to_tuple  
+                            (fun (x : Core.type) (X : Core.eval_type x) => X)
+                            exprs
+                  in
+                    Core.builtin_denotation args res f exprs
+              | Emux t b x y => if b then x else y 
+              | Econstant ty c => c
+              | Etuple l exprs => 
+                  Common.DList.to_tuple (fun _ X => X) exprs
+              | Enth l t v e => 
+                  Common.Tuple.get _ _ v e
+              | Efst l t  e => 
+                  Common.Tuple.fst e
+              | Esnd l t  e => 
+                  Common.Tuple.snd e
+            end 
+        in eval_expr t e).  
+    Defined. 
+        
+    Definition eval_effects (e : effects Core.eval_type) (Delta : updates) : updates.  
     unfold effects in e. 
-
-    (* refine (Tuple.fold Phi _ e Delta).  *)
-    refine (DList.map3 _ Phi e st Delta). 
-
-    Definition eval_effect (a : sync) :   
-      (option ∘ effect eval_type) a ->
-      eval_sync a -> (option ∘ eval_sync) a -> (option ∘ eval_sync) a. 
+    
+    (* refine (DList.fold Phi _ e Delta).  *)
+    refine (Common.DList.map3 _ Phi e st Delta). 
+    Import Common Core.
+    Definition eval_effect (a : Core.sync) :   
+      (Common.comp option (effect Core.eval_type)) a ->
+      Core.eval_sync a -> (Common.comp option Core.eval_sync) a -> (Common.comp option Core.eval_sync) a. 
     
     refine (fun  eff => 
               match eff with 
-                  | Some eff =>  
-                      match eff in effect _ s return eval_sync s -> (option ∘ eval_sync) s -> (option ∘ eval_sync) s  with 
-                        |  effect_reg_write t val we =>  fun _ old => 
+                | Some eff =>  
+                    match eff in effect _ s return eval_sync s -> (option ∘ eval_sync) s -> (option ∘ eval_sync) s  with 
+                      |  effect_reg_write t val we => 
+                           fun _ old => 
                              match old with 
                                | Some _ => old
                                | None => if we then Some val else None
                              end
-                        |  effect_regfile_write n t val adr we => fun rf old =>
+                      |  effect_regfile_write n t val adr we => 
+                           fun rf old =>
                              match old with 
                                | Some _ => old 
                                | None => 
@@ -352,532 +226,140 @@ Section t.
                                    else 
                                      None                                       
                              end
-                      end
-                  | None => fun _ old => old            
-            end). 
+                    end
+                | None => fun _ old => old            
+              end). 
     Defined. 
     apply eval_effect. 
     Defined. 
-
-    Fixpoint eval_block t  (T : block eval_type t) :
-      updates -> option (eval_type t * updates) := 
-      match T with
-        | telescope_bind arg bind cont => 
-            fun Delta => 
-              let res := eval_bind _ bind in
-              eval_block _ (cont res) Delta
-        | telescope_end (p, g, e) => fun Delta =>
-                                      let g := eval_expr _ g  in             
-                                      if g then                                         
-                                        Some (p, eval_effects e Delta)
-                                      else None
-    end. 
-  
-     
-  End sem. 
-  
-  Section correctness. 
-  
     
-    Notation C := (compile_inner eval_type tt). 
-    Lemma eval_andb_true x y : (eval_expr Tbool (andb eval_type x y)) = (eval_expr Tbool x && eval_expr Tbool y)%bool.
-    Proof. 
-      Import Equality Bool. 
-      
-      dependent destruction x; dependent destruction y; simpl;
-      repeat match goal with 
-                 c : constant B |- _ => destruct c
-               | x : eval_type Tbool |- _ => destruct x
-               | _ => idtac
-             end; rewrite ?andb_true_r, ?andb_true_l, ?andb_false_l , ?andb_false_r ; reflexivity.  
-    Qed. 
+    Fixpoint eval_telescope { A B} (F : A -> B) (T : telescope  eval_type A) :=
+      match T with 
+        | telescope_end X => F X
+        | telescope_bind arg bind cont =>
+            let res := eval_expr arg bind in 
+              eval_telescope F (cont res)
+      end. 
+    
+    Definition eval_block  t  (T : block eval_type t) Delta :
+      option (eval_type t * updates) := 
+      eval_telescope (fun x => match x with (p,g,e)  =>
+                                             if g : bool then                              
+                                               Some (p, eval_effects e Delta)
+                                             else None end) T. 
+  End sem.
+End t.  
 
-    Lemma eval_orb_true x y : (eval_expr Tbool (orb eval_type x y)) = (eval_expr Tbool x || eval_expr Tbool y)%bool.
-    Proof. 
-      Import Equality Bool. 
-      
-      dependent destruction x; dependent destruction y; simpl;
-      repeat match goal with 
-                 c : constant B |- _ => destruct c
-               | x : eval_type Tbool |- _ => destruct x
-               | _ => idtac
-             end; rewrite ?orb_true_r, ?orb_true_l, ?orb_false_l , ?orb_false_r ; reflexivity.  
-    Qed. 
+Notation "e :-- t1 ; t2 " := (compose _ _  t1 (fun e => t2)) (right associativity, at level 80, e1 at next level).
+Notation "x :- e1 ; e2" := (telescope_bind _ _ _ _ (e1) (fun x => e2)) (right associativity, at level 80, e1 at next level).  
+Notation " & e " := (telescope_end _   _ _ e) (at level 71). 
 
 
-    Lemma eval_neffects_append  st e f (Delta : updates) : 
-      eval_neffects st (e ++ f) Delta = 
-                   eval_neffects st f (eval_neffects st e Delta).              
-    Proof. 
-      revert Delta. 
-      induction e. 
-      + reflexivity. 
-      + intros Delta.
-        
-        simpl. rewrite IHe. reflexivity.  
-    Qed. 
-
-    Variable st : eval_state Phi. 
-
-    Notation "B / Delta " := (eval_nblock st _ B Delta). 
-    Theorem CPS_compile_correct t (a : action Phi eval_type t)  Delta:
-      eval_nblock st _ (C t a ) Delta =  (Front.Sem.eval_action a st Delta).
-    Proof. 
-      revert Delta. 
-      induction a. 
-      - intros.  reflexivity. 
-      - intros Delta. simpl. unfold  Sem.Dyn.Bind. rewrite <- IHa.
-        transitivity (
-            do ed <- (C t a) / Delta ; 
-            let (e,d) := ed in 
-              eval_nblock st u (C u (f e)) d
-                   ); 
-        [|destruct  ((C t a) / Delta) as [[ e d ]| ]; simpl; easy]. 
-        clear IHa H.
-        generalize (C t a) as T. intros T. clear a.
-        
-        induction T. destruct a as [[rA gA] eA]. 
-        simpl in *. 
-        case_eq (eval_expr Tbool gA); intros H.  simpl.
-        unfold compose_block; simpl compose.  
-        induction (C u (f rA)). simpl. destruct a as [[rB gB] eB]. simpl. 
-        * rewrite eval_neffects_append. rewrite eval_andb_true. rewrite H. simpl. reflexivity. 
-        * simpl. rewrite H0. reflexivity.         
-
-        * unfold compose_block. simpl. induction (C u (f rA)). destruct a as [[rB gB] eB]. simpl. 
-          rewrite eval_andb_true. rewrite H. reflexivity.  
-          simpl. rewrite H0. reflexivity. 
-        * unfold compose_block. simpl. unfold compose_block in H. rewrite H. reflexivity.
-
-      - simpl. intros. 
-          Ltac t :=
-            repeat match goal with 
-                     | |- context [check ?x ; ?y] => 
-                         let H := fresh "check" in 
-                           case_eq x; intros H
-                   end. 
-          t; trivial. 
-      -                         (* primitive *)
-      intros. destruct p.  
-        +  simpl. reflexivity. 
-        + simpl.
-              
-          set (x := DList.to_tuple eval_expr exprs). 
-          replace (x) with (fst x, snd x) by (destruct x; reflexivity).
-          simpl.
-          DList.inversion. simpl. reflexivity. 
-
-        + simpl. 
-          DList.inversion; reflexivity.
-        + simpl. repeat DList.inversion. simpl. reflexivity.
-          Arguments andb R _ _ : simpl never. 
-          Arguments orb R _ _ : simpl never. 
-          Ltac s :=
-            match goal with 
-              |- context [eval_expr _ (orb _ ?x ?y )] => rewrite eval_orb_true
-            | |- context [eval_expr _ (andb _ ?x ?y )] => rewrite eval_andb_true
-            | H : context [eval_expr _ (orb _ ?x ?y )] |- _ => rewrite eval_orb_true in H
-            | H : context [eval_expr _ (andb _ ?x ?y )] |- _  => rewrite eval_andb_true in H
-            | H : eval_expr _ ?x = true |- context [eval_expr _ ?x] => rewrite H
-            | H : eval_expr _ ?x = true , H' : context [eval_expr _ ?x] |- _ => rewrite H in H'
-            | H : eval_expr _ ?x = false |- context [eval_expr _ ?x] => rewrite H
-            | H : eval_expr _ ?x = false , H' : context [eval_expr _ ?x] |- _ => rewrite H in H'
-            end. 
-      - intros. simpl.   unfold Sem.Dyn.OrElse. 
-        rewrite <- IHa1, <- IHa2 . clear IHa1 IHa2. 
-        generalize (C t a1); intros T; generalize (C t a2); intros T'. 
-        induction T as [[[rA gA] eA] |]; simpl.
-        induction T' as [[[rA' gA'] eA'] |]. simpl compose.
-        t. simpl. repeat (s; simpl). reflexivity. 
-        t. simpl. repeat (s; simpl). t. reflexivity. 
-        reflexivity. 
-        simpl. unfold compose_block in *. simpl in *.  rewrite H. reflexivity. 
-        simpl. unfold compose_block in *. simpl in *.  rewrite H. reflexivity. 
-
-    Qed.
-     
-  End correctness.     
- End t. 
-
-Section correctness2. 
+Section correctness. 
+  Import Equality.
   
-  Notation Cs  := (compile_neffects  _ _).
-  Notation C  := (compile_neffect  _ _).
-  Notation "x <- e1 ; e2" := (@telescope_bind _ _ _ _ _ e1 (fun x => e2)) (right associativity, at level 80, e1 at next level).
-  Notation " & e " := (@telescope_end _ _ _ e) (at level 71).
-  Notation "e :- t1 ; t2 " := (@compose  _ _ _ _ t1 (fun e => t2)) (right associativity, at level 80, t1 at next level).
-
-  
-
-  Ltac t := simpl; intuition; try match goal with
-                                    | [ H : _ |- _ ] => rewrite H; auto
-                                end.
-   
-  
-  Lemma eval_effect_init Phi st Delta : eval_effects Phi st (init_effects Phi eval_type) Delta = Delta. 
-  Proof.
-    unfold eval_effects. 
-    induction Phi. simpl. reflexivity. 
-    simpl. repeat DList.inversion. simpl. f_equal. apply IHPhi. 
+  Lemma compile_effects_correct Phi st   e : 
+    forall Delta, 
+      eval_effects Phi st (compile_effects Phi Core.eval_type e) Delta =
+                 IR.eval_effects Phi st e Delta. 
+  Proof. 
+    induction Phi. simpl. auto. 
+    simpl; intros. unfold IR.effects in e. repeat DList.inversion. 
+    case_eq c; intros; simpl; subst;
+    destruct x1.
+    dependent destruction e0. simpl. 
+    rewrite IHPhi; reflexivity.
+    simpl; f_equal; auto. 
+    simpl; f_equal; auto. 
+    simpl; f_equal; auto.
+    destruct e. simpl. reflexivity.
+    simpl. reflexivity. 
+    simpl. f_equal. auto. 
   Qed. 
-
+  
+  Hint Resolve compile_effects_correct. 
+  
   Lemma foo {Phi R A B C} (T: telescope Phi R A) (f : A -> telescope  Phi R B)  (g : B -> telescope Phi R C) :
-    (X :- (Y :- T; f Y); (g X) )= (Y :- T; X :- f Y; g X).
+    (X :-- (Y :-- T; f Y); (g X) )= (Y :-- T; X :-- f Y; g X).
   Proof.
-      induction T. reflexivity. simpl.
-      f_equal.
-      Require Import  FunctionalExtensionality.
-      apply functional_extensionality.
-      apply H.
-  Qed.
-     
-  Lemma my_ind Phi (R : type -> Type) (P : neffect Phi R -> Prop) :
-    (forall (guard : expr R Tbool) ,
-       P (neffect_guard Phi  R guard [])) ->
-    (forall (guard : expr R Tbool) a l ,
-       P a -> P (neffect_guard Phi  R guard l) ->
-       P (neffect_guard Phi  R guard (a :: l))) ->
-    (forall (t : type) (v : var Phi (Treg t)) (r : R t),
-       P (neffect_reg_write  Phi R t v r)) ->
-    (forall (n : nat) (t : type) (v : var Phi (Tregfile n t))
-       (r : R ( (Tint n))) (r0 : R t),
-       P (neffect_regfile_write Phi R n t v r r0)) ->
-    forall n : neffect Phi R, P n. 
-  Proof.
-    intros. 
-    refine (let fold := fix fold n :=
-        match n with
-            | neffect_guard g l => 
-                let fix foldi l : P (neffect_guard Phi R g l) :=
-                    match l return  P (neffect_guard Phi R g l) with 
-                      | nil => H g
-                      | cons t q => H0 g t q (fold t) (foldi q)
-                    end in foldi l
-            | neffect_reg_write t v w => H1 t v w
-            | neffect_regfile_write n t v adr w => H2 n t v adr w
-        end in fold n). 
-  Qed. 
-  
-  Lemma correspondance Phi l e : forall g1 g2, 
-                               compile_neffect Phi eval_type g1 (neffect_guard Phi eval_type g2 l) e = (compile_neffects Phi eval_type (andb _ g1  g2)%expr l e).
-  Proof.                                                                                        
-    induction l; reflexivity.
-  Qed. 
-  
-  Lemma eval_neffect_cons Phi st guard a l Delta: 
-    eval_neffect Phi st (neffect_guard Phi eval_type guard (a :: l)) Delta = 
-                 (if eval_expr Tbool guard
-                  then eval_neffects Phi st l (eval_neffect Phi st a Delta)
-                  else Delta).
-  Proof. 
-    reflexivity. 
+    induction T. reflexivity. simpl.
+    f_equal.
+    Require Import  FunctionalExtensionality.
+    apply functional_extensionality.
+    apply H.
   Qed.
   
-  Fixpoint eval_telescope { A B} Phi st (F : A -> B) (T : telescope  Phi eval_type A) :=
-    match T with 
-      | telescope_end X => F X
-      | telescope_bind arg bind cont =>
-          let res := eval_bind Phi st arg bind in 
-            eval_telescope Phi st F (cont res)
-    end. 
-
-  Lemma folder Phi st guard l Delta: eval_neffect Phi st (neffect_guard  Phi eval_type guard l) Delta 
-                                         = if eval_expr Tbool guard then eval_neffects Phi st l Delta else Delta.
-  Proof. 
-    reflexivity. 
-  Qed. 
+  
+  Section compile_expr. 
+    Context {A B : Type}. 
+    Context {E : A -> B}.  
+    Variable (Phi : Core.state) (st : Core.eval_state Phi). 
+    Notation Ev := (eval_telescope Phi st E). 
     
-
-  
-  Notation "[[ x ]]" := (eval_expr Tbool x). 
-  Arguments Tuple.set {T F l t} _ _ _.
-  Arguments Tuple.get {T F l t} _ _. 
-
-  Notation Ev Phi st  := (eval_telescope Phi st (eval_effects Phi st)).  
-  
-  Ltac v := match goal with 
-                |- context [match ?X with  | ( _ , _  )  => _ end ] => destruct X 
-            end. 
-  Import Equality. 
-  Ltac d := match goal with 
-              | H : context [match ?X with | _ => _ end] |- _ => dependent destruction X
-              |  |- context [match ?X with | _ => _ end] => case_eq  X; intros; subst; simpl
-                                                                                      
-            end. 
-
-  Lemma rew_1 Phi st Delta t (v : var Phi t ) x e : 
-    eval_effects Phi st (DList.set v (Some x) e) Delta =
-                 DList.set v (eval_effect t (Some x) (DList.get v st) (DList.get v Delta))  (eval_effects Phi st e Delta).  
-  Proof. 
-    induction Phi; [dependent destruction v|]. 
-    dependent destruction v. 
-    simpl; repeat v; destruct x; simpl; d; f_equal.
-    simpl. repeat v; destruct x; simpl; rewrite IHPhi; clear IHPhi; 
-           simpl; repeat d; simpl in *; auto. 
-  Qed. 
-
-  Lemma inversion_1 Phi st : forall t (v : var Phi (Treg t)) e Delta x x', 
-                             inversion_effect_Treg eval_type t x = (x', true) ->
-                             DList.get v e = Some x ->
-                             exists y, DList.get v (eval_effects Phi st e Delta) = Some y.
-  Proof. 
-    induction Phi; [dependent destruction v|]. 
-    dependent destruction v; simpl; intros. 
-    repeat v; dependent destruction x; simpl in *; inversion H; subst; clear H; simpl.
-    repeat DList.inversion.  simpl in H0. subst. simpl.
-    d; eauto.
-
-    simpl in *. repeat v. simpl. edestruct IHPhi; eauto.
-  Qed. 
-
-
-  Lemma compile_effect_correct Phi st a  : 
-    forall Delta e g , 
-      eval_telescope Phi st (eval_effects Phi st) (C g a e) Delta 
-                     =  if [[g]] then eval_neffect Phi st a (Ev Phi st (&e) Delta) else (Ev Phi st (&e)Delta). 
-  Proof. 
-      induction a using my_ind. 
-      - intros. simpl. destruct ([[guard]]); destruct ([[g]]); reflexivity.
-      - intros. rewrite correspondance. rewrite eval_neffect_cons. 
-        simpl compile_neffects. simpl.
-        setoid_rewrite correspondance in IHa0.
-        
-        revert IHa IHa0.
-        intros H. specialize (H Delta e (andb _ g guard)%expr). revert H. 
-        induction (C (andb _ g guard)%expr a e); intros. 
-        {simpl. rewrite IHa0. rewrite folder. simpl. simpl in H. rewrite eval_andb_true in H.        simpl in H. 
-         destruct ([[g]]); destruct ([[guard]]); simpl; simpl in H; try rewrite H; try reflexivity. }
-         {
-         simpl. rewrite H. reflexivity. 
-         simpl. simpl in *. rewrite H0. reflexivity.
-         apply IHa0.          
-         }
-      - intros. simpl.
-        unfold update. 
-        case_eq (DList.get  v e); intros; simpl. 
-        +               
-        (* case: there was a previous effect on this register *)
-        case_eq (inversion_effect_Treg eval_type t e0); intros; simpl.       
-          
-        
-        rewrite rew_1. 
-        case_eq (e2); intros; simpl. 
-          * destruct ([[g]]). 
-            subst. 
-            {
-              Lemma hint_1 Phi : forall st t (v : var Phi (Treg t)) r Delta e  e0, 
-                                 DList.get v e = Some e0 -> 
-                                 forall e1, inversion_effect_Treg eval_type t e0 = (e1, true) -> 
-                                       DList.set v
-                                            match DList.get v Delta with
-                                                | Some _ => DList.get v Delta
-                                                | None => Some e1
-              end (eval_effects Phi st e Delta) =
-                                          Diff.add Phi (eval_effects Phi st e Delta) (Treg t) v r. 
-              Proof. 
-                
-                induction Phi; [dependent destruction v|].
-                simpl. intros; repeat v. 
-                 dependent destruction v; simpl; intros. 
-                 unfold eval_state in *; repeat DList.inversion.  
-                 unfold Diff.add;  simpl; repeat d; simpl in *; subst;
-                 simpl in H1; dependent destruction e0; f_equal; auto.
-                 discriminate. 
-                 simpl in *; inversion H0; subst; auto. 
-                 simpl in *; inversion H0; subst; discriminate.
-                 simpl in *. setoid_rewrite IHPhi. unfold Diff.add.  simpl.
-                 repeat d; reflexivity.
-                 eauto. 
-                 eauto. 
-              Qed.
-            eapply hint_1; eauto. 
-            }
-            subst.
-            {
-              induction Phi; [dependent destruction v|]. 
-              simpl; repeat v. 
-              dependent destruction v; simpl in *; subst. unfold Diff.add.
-              unfold eval_state in *; unfold effects in *.  repeat DList.inversion. simpl in *.
-              repeat d; clear IHPhi; dependent destruction e0;subst; f_equal; auto. 
-              simpl in H0. inversion H0; subst. auto.
-              simpl. rewrite IHPhi. auto. auto. 
-            }
-         
-            
-
-          * subst.
-            destruct ([[g]]). 
-            simpl. 
-            unfold Diff.add. 
-            {
-            induction Phi; [dependent destruction v|]. 
-              simpl; repeat v. 
-              dependent destruction v; simpl in *; subst. unfold Diff.add.
-              unfold eval_state in *; unfold effects in *.  repeat DList.inversion. simpl in *.
-
-              repeat d; clear IHPhi; dependent destruction e0;subst; f_equal; auto. 
-              discriminate. simpl in *; inversion H0; subst; auto. 
-              simpl in *; inversion H0; subst; auto. 
-              discriminate.
-              
-              setoid_rewrite IHPhi. clear IHPhi. unfold Diff.add. simpl. d. reflexivity.
-              reflexivity. 
-              auto. 
-            }
-            
-            {
-            induction Phi; [dependent destruction v|]. 
-              simpl; repeat v. 
-              dependent destruction v; simpl in *; subst. unfold Diff.add.
-              unfold eval_state in *; unfold effects in *.  repeat DList.inversion. simpl in *.
-
-              repeat d; clear IHPhi; dependent destruction e0;subst; f_equal; auto. 
-              simpl in *. inversion H0; auto. 
-              
-              setoid_rewrite IHPhi. auto.  auto. 
-            
-            }
-            
-            
-            
-        + rewrite rew_1. simpl. 
-
-          unfold Diff.add. 
-          {
-          
-            induction Phi; [dependent destruction v|]. 
-              simpl; repeat v. 
-              dependent destruction v; simpl in *; subst. unfold Diff.add.
-              unfold eval_state in *; unfold effects in *.  repeat DList.inversion. simpl in *.
-repeat d; repeat f_equal. 
-              
-              setoid_rewrite IHPhi. clear IHPhi. unfold Diff.add. simpl. repeat d; f_equal. auto. 
-          }
-
-      - intros. simpl.         unfold update. 
-        case_eq (DList.get v e); intros; simpl. 
-        +               
-        case_eq (inversion_effect_Tregfile eval_type t n e0); intros [w adr we H']; simpl.         
-        rewrite rew_1.
-        simpl.
-        case_eq (we); intros; simpl. 
-        * destruct [[g]]. 
-          unfold Diff.add.
-          {
-            induction Phi; [dependent destruction v|].
-            simpl; repeat v. 
-            dependent destruction v; simpl in *; subst.
-            unfold eval_state in *; unfold effects in *.  repeat DList.inversion. simpl in *; subst. 
-            
-
-            unfold Diff.add; repeat d; repeat f_equal; dependent destruction e0; simpl in H'; inversion H'; subst;  try congruence; try simpl in *; try auto.
-            rewrite IHPhi; clear IHPhi;  auto. 
-            unfold Diff.add; repeat d; repeat f_equal; dependent destruction e0; simpl in H'; inversion H'; subst;  try congruence; try simpl in *; try auto.
-          }
-          subst. 
-          {
-            induction Phi; [dependent destruction v|].
-            simpl; repeat v. 
-            dependent destruction v; simpl in *; subst. 
-            unfold eval_state in *; unfold effects in *.  repeat DList.inversion. simpl in *; subst. 
-
-            unfold Diff.add; repeat d; repeat f_equal; dependent destruction e0; simpl in H'; inversion H'; subst;  try congruence; try simpl in *; try auto.
-            rewrite IHPhi; clear IHPhi;  auto. 
-          }
-
-          *destruct [[g]]. subst. 
-          unfold Diff.add. 
-          {
-              induction Phi; [dependent destruction v|].
-            simpl; repeat v. 
-            dependent destruction v; simpl in *; subst. 
-                        unfold eval_state in *; unfold effects in *.  repeat DList.inversion. simpl in *; subst. 
-unfold Diff.add; repeat d; repeat f_equal; dependent destruction e0; simpl in H'; inversion H'; subst;  try congruence; try simpl in *; try auto.
-            rewrite IHPhi; clear IHPhi;  auto. 
-            repeat d; repeat f_equal; dependent destruction e0; simpl in H'; inversion H'; subst;  try congruence; try simpl in *; try auto.          
-          }
-          {
-            induction Phi; [dependent destruction v|].
-            simpl; repeat v. 
-            dependent destruction v; simpl in *; subst. unfold Diff.add.
-                        unfold eval_state in *; unfold effects in *.  repeat DList.inversion. simpl in *; subst. 
-repeat d; repeat f_equal; dependent destruction e0; simpl in H'; inversion H'; subst;  try congruence; try simpl in *; try auto.
-            rewrite IHPhi; clear IHPhi; auto. }
-          
-          
-        + rewrite rew_1. simpl.
-          unfold Diff.add. 
-          {
-            induction Phi; [dependent destruction v|].
-            simpl; repeat v. 
-            dependent destruction v; simpl in *; subst. unfold Diff.add.
-            unfold eval_state in *; unfold effects in *.  repeat DList.inversion. simpl in *; subst. 
-
-            repeat d; repeat f_equal; dependent destruction e0; simpl in H'; inversion H'; subst;  try congruence; try simpl in *; try auto.
-            rewrite IHPhi; clear IHPhi; auto. 
-            repeat d; repeat f_equal; dependent destruction e0; simpl in H'; inversion H'; subst;  try congruence; try simpl in *; try auto. 
-
-          }
-    Qed. 
-
-    Lemma eval_telescope_neffects Phi st es : forall Delta e g, eval_telescope Phi st (eval_effects Phi st) (Cs g es e) Delta 
-                               =  if [[g]] then eval_neffects Phi st es (Ev Phi st (&e) Delta) else Ev Phi st (&e) Delta. 
+    Section compile_exprs. 
+      Notation P := (fun t e => 
+                       forall  (f : Core.eval_type t -> telescope _ _ A), 
+                         Ev(r :-- compile_expr Phi Core.eval_type t e; f r) = 
+                           Ev (f (Front.eval_expr t e))). 
+      Lemma compile_exprs_correct : forall l dl f,         
+                                      Common.DList.Forall P dl ->                    
+                                      Ev (Y :-- compile_exprs Phi Core.eval_type l dl; f Y) =
+                                         Ev (f (Common.DList.map Front.eval_expr dl )). 
+      Proof. 
+        induction dl. simpl. reflexivity. 
+        simpl. intros. rewrite foo. destruct H. rewrite H. rewrite foo. simpl. apply IHdl. auto. 
+      Qed. 
+    End compile_exprs. 
+    Lemma compile_expr_correct t e (f : Core.eval_type t -> telescope _ _ A): 
+      Ev (r :-- compile_expr Phi Core.eval_type t e; f r) = Ev (f (Front.eval_expr t e)). 
     Proof. 
-      induction es. 
-      intros; simpl.  destruct ([[g]]); reflexivity.  
-      simpl. intros. 
-      pose (H := compile_effect_correct Phi st a Delta e g). 
-      clearbody H. revert H. 
-      induction (C g a e). 
-      - simpl.       intros H. 
-      rewrite IHes. simpl. rewrite H. destruct ([[g]]); reflexivity.
-      - simpl. intros. apply H. simpl. auto.  
-    Qed. 
- 
-    Theorem nblock_compile_correct Phi (st : eval_state Phi) t (nb : nblock Phi eval_type t)  Delta:
-      eval_block Phi st _  (nblock_to_block Phi eval_type nb) Delta =  eval_nblock Phi st _ nb Delta. 
-      unfold nblock in nb. 
-      induction nb as [ [ [rA gA] eA]|]. 
-      2: simpl; rewrite <- H; reflexivity. 
+      revert e.
+      induction e using Front.expr_ind_alt; try reflexivity. 
       
-      {
-        unfold nblock_to_block. unfold compose_block. simpl.
-        pose (H := eval_telescope_neffects Phi st eA Delta (init_effects Phi eval_type) gA). 
-        clearbody H. 
-        case_eq ([[gA]]).
-        {
-          intros. rewrite H0 in H. simpl in H. 
-          rewrite eval_effect_init in H. 
-          rewrite <- H. clear H.  
-          induction (Cs gA eA (init_effects Phi eval_type)). simpl. rewrite H0. reflexivity. 
-          simpl. rewrite <- H. reflexivity. 
-        }
-        {
-          intros.
-          induction (Cs gA eA (init_effects Phi eval_type)). simpl. rewrite H0. reflexivity. 
-          simpl. apply H1. auto.          
-        }
-      }
-
+      Ltac t :=
+        match goal with 
+            |- context [ (_ :-- _ :-- _; _ ; _) ] => rewrite foo
+          | H : context [ _ :-- _ ; _ ] |- _ => rewrite H ; clear H
+      end.
+      
+      { simpl. rewrite (compile_exprs_fold Phi Core.eval_type). repeat rewrite foo; simpl.
+        rewrite compile_exprs_correct; auto.  simpl.  repeat f_equal. 
+        rewrite Common.DList.map_to_tuple_commute. reflexivity. }       
+      
+      {simpl; repeat t; reflexivity.   }
+      {simpl; repeat t; reflexivity.   }
+      {simpl; repeat t; reflexivity.   }
+      {simpl; repeat t; reflexivity.   }
+      
+      { simpl. rewrite (compile_exprs_fold Phi Core.eval_type). repeat rewrite foo; simpl.
+        rewrite compile_exprs_correct; auto.  simpl.  repeat f_equal.
+        
+        rewrite Common.DList.map_to_tuple_commute. reflexivity. }       
+    
     Qed. 
+  End compile_expr. 
   
-End correctness2. 
-
-Definition Block Phi t := forall V,  block Phi V t. 
-Definition Compile Phi t (A : forall V, action Phi V t) : Block Phi t := 
-  fun V =>
-    nblock_to_block Phi V (compile Phi V t (A V)):block Phi V t. 
-Definition Eval Phi st t (B : Block Phi t) Delta :=
-  eval_block Phi st t (B _) Delta. 
-
-
-Theorem Compile_correct Phi t A : forall st Delta,
-  Eval Phi st t (Compile Phi t A) Delta =  Front.Eval Phi st t A Delta. 
-Proof. 
-  unfold Compile, Eval, Front.Eval. intros. 
-  rewrite nblock_compile_correct. 
-  simpl.  rewrite CPS_compile_correct. reflexivity.   
-Qed. 
+  Lemma compile_correct Phi st t (b : IR.block Phi Core.eval_type t) : 
+    forall Delta, 
+      eval_block Phi st t (compile Phi Core.eval_type t b) Delta = IR.eval_block Phi st t b Delta. 
+  Proof. 
+    intros.
+    induction b.
+    simpl. destruct a as [[r g] e]; simpl.
+    unfold eval_block. 
+    
+    
+    rewrite (compile_expr_correct Phi st Core.Tbool g). simpl. 
+    destruct (Front.eval_expr Core.Tbool g); repeat f_equal.
+    
+    apply compile_effects_correct. 
+    
+    simpl. rewrite <- H. clear H. 
+    unfold eval_block. destruct b; try reflexivity. 
+    
+    rewrite (compile_expr_correct Phi st arg e) . reflexivity.  
+  Qed. 
+End correctness. 
 
 
 Section equiv. 
@@ -892,31 +374,34 @@ Section equiv.
   Variable R : forall t, U t -> V t -> Prop. 
   Notation "x -- y" := (R _ x y) (at level 70, no associativity). 
     
-  Inductive expr_equiv : forall t,  expr U t -> expr  V t -> Prop :=
-  | Eq_var : forall  t (v1 : U t) v2, v1 -- v2 -> Evar v1 == Evar v2
+  Inductive expr_equiv : forall t,  expr Phi U t -> expr Phi V t -> Prop :=
+  | Eq_read : forall t v, Eread Phi U t v == Eread Phi V t v
+  | Eq_read_rf : forall n t v adr1 adr2, 
+                   adr1 -- adr2 -> 
+                   Eread_rf Phi U n t v adr1 == Eread_rf Phi V n t v adr2
   | Eq_builtin : forall args res (f : builtin args res) dl1 dl2, 
-                   Common.DList.pointwise expr_equiv args dl1 dl2 ->
-                   Ebuiltin  f dl1 == Ebuiltin  f dl2
-  | Eq_constant : forall ty (c : constant ty), Econstant c == Econstant c
+                   Common.DList.pointwise R args dl1 dl2 ->
+                   Ebuiltin Phi U args res f dl1 == Ebuiltin Phi V args res f dl2
+  | Eq_constant : forall ty c, Econstant Phi U ty c == Econstant Phi V ty c
   | Eq_mux : forall t c1 c2 l1 l2 r1 r2, 
-               c1 == c2 -> l1 == l2 -> r1 == r2 -> 
-               Emux  U t c1 l1 r1 ==  Emux  V t c2 l2 r2
+               c1 -- c2 -> l1 -- l2 -> r1 -- r2 -> 
+               Emux Phi U t c1 l1 r1 ==  Emux Phi V t c2 l2 r2
                     
   | Eq_fst : forall (l : list type) (t : type) dl1 dl2, 
-               dl1 == dl2 -> 
-               Efst  U l t dl1 == Efst  V l t dl2
+               dl1 -- dl2 -> 
+               Efst Phi U l t dl1 == Efst Phi V l t dl2
 
   | Eq_snd : forall (l : list type) (t : type) dl1 dl2, 
-               dl1 == dl2 -> 
-               Esnd  U l t dl1 == Esnd  V l t dl2
+               dl1 -- dl2 -> 
+               Esnd Phi U l t dl1 == Esnd Phi V l t dl2
 
   | Eq_nth : forall (l : list type) (t : type) (v : Common.var l t)  dl1 dl2, 
-               dl1 == dl2 -> 
-               Enth v dl1 == Enth v dl2
+               dl1 -- dl2 -> 
+               Enth Phi U l t v dl1 == Enth Phi V l t v dl2
 
   | Eq_tuple : forall (l : list type) dl1 dl2, 
-                 Common.DList.pointwise expr_equiv l dl1 dl2 ->
-               Etuple  U l dl1 == Etuple  V l dl2
+                 Common.DList.pointwise R l dl1 dl2 ->
+               Etuple Phi U l dl1 == Etuple Phi V l dl2
                             where "x == y" := (expr_equiv _ x y). 
   
   Inductive effect_equiv : forall t,  option (effect U t) -> option (effect V t) -> Prop :=
@@ -932,7 +417,7 @@ Section equiv.
  
   Definition effects_equiv : effects Phi U -> effects Phi V -> Prop := 
     Common.DList.pointwise  effect_equiv Phi. 
-  
+    
   End inner_equiv. 
  
   Inductive Gamma : Type :=
@@ -951,23 +436,97 @@ Section equiv.
   Reserved Notation "G |- x ==b y" (at level 70, no associativity). 
   Notation "G |- x -- y" := (In _ x y G) (at level 70, no associativity). 
 
-  Inductive bind_equiv t : forall (G : Gamma), bind Phi U t -> bind Phi V t -> Prop :=
-  |Eq_expr : forall G v1 v2, expr_equiv (R G) t v1 v2 ->
-                        bind_equiv t G (bind_expr Phi U t v1) (bind_expr Phi V t v2)
-  |Eq_reg : forall G v, bind_equiv t G  (bind_reg_read Phi U t v) (bind_reg_read Phi V t v)
-  |Eq_regfile : forall G n v a1 a2, 
-                  G |- a1 -- a2 ->
-                  bind_equiv t G  (bind_regfile_read Phi U t n v a1) (bind_regfile_read Phi V t n v a2). 
-
   Inductive block_equiv t : forall (G : Gamma), block Phi U t -> block Phi V t -> Prop :=
   | Eq_end : forall G (v1 : U t) v2 g1 g2 e1 e2, 
-               G |- v1 -- v2 ->  expr_equiv (R G) _ g1 g2 -> effects_equiv (R G) e1 e2 ->
+               G |- v1 -- v2 -> G |- g1 -- g2 -> effects_equiv (R G) e1 e2 ->
                G |- telescope_end Phi U _ (v1, g1, e1) ==b telescope_end Phi V _ (v2,g2, e2 ) 
-  | Eq_bind : forall G a (e1 : bind Phi U a) e2 (k1 : U a -> block Phi U t) k2,
-                bind_equiv _ G e1 e2 -> 
+  | Eq_bind : forall G a (e1 : expr Phi U a) e2 (k1 : U a -> block Phi U t) k2,
+                expr_equiv (R G) _ e1 e2 -> 
                 (forall v1 v2, (* G |- v1 -- v2 ->  *)cons _ v1 v2 G |- k1 v1 ==b k2 v2) ->
                 G |- telescope_bind Phi U _ a e1 k1 ==b telescope_bind Phi V _ a e2 k2                
                  where "G |- x ==b y" := (block_equiv _ G x y). 
 End equiv. 
 
+Definition Block Phi t := forall V, block Phi V t. 
 Definition WF Phi t (b : Block Phi t) := forall U V, block_equiv U V Phi t (nil _ _) (b _) (b _). 
+Definition Compile Phi t (B : IR.Block Phi t) : Block Phi t :=
+  fun V => compile _ _ _ (B _).  
+Definition Eval Phi st t (B : Block Phi t) Delta :=
+  eval_block Phi st t (B _) Delta. 
+
+Theorem Compile_correct Phi t b : forall st Delta,
+  Eval Phi st t (Compile Phi t b) Delta =  IR.Eval Phi st t b Delta. 
+Proof. 
+  unfold Eval, Compile. intros. apply compile_correct.
+Qed. 
+(*
+Require Import Eqdep. 
+Ltac t :=  subst; repeat match goal with 
+                       H : existT _ _ _ = existT _ _ _ |- _ => 
+                         apply Eqdep.EqdepTheory.inj_pair2 in H
+                   |   H : context [eq_rect ?t _ ?x ?t ?eq_refl] |- _ => 
+                         rewrite <- eq_rect_eq in H
+                   |   H : context [eq_rect ?t _ ?x ?t ?H'] |- _ => 
+                         rewrite (UIP_refl _ _ H') in H;
+                         rewrite <- eq_rect_eq in H
+                   |   H : existT _ ?t1 ?x1 = existT _ ?t2 ?x2 |- _ => 
+                         let H' := fresh "H'" in 
+                           apply eq_sigT_sig_eq in H; destruct H as [H H']; subst
+                         end; subst.
+
+Theorem Compile_wf Phi t b : IR.WF Phi t b -> WF Phi t (Compile Phi t b). 
+Proof. 
+  unfold IR.WF, WF. 
+  intros. specialize (H U V).
+  unfold Compile.
+  Record rel U V G G' :=
+    {
+      rel_1 :  (forall t v1 v2, IR.In U V t v1 v2 G -> In U V t v1 v2 G')
+    }. 
+  Hint Resolve rel_1. 
+  Lemma compile_effects_wf Phi U V G  : 
+    forall e1 e2,
+      IR.effects_equiv U V Phi (fun t x y => IR.In U V t x y G) e1 e2 ->
+      forall G', 
+        rel U V G G' ->
+        effects_equiv U V Phi (fun t x y => In U V t x y G') 
+                      (compile_effects Phi U e1) (compile_effects Phi V e2). 
+  Proof. 
+  Admitted.
+  Hint Resolve compile_effects_wf.
+  Hint Unfold R. 
+  Lemma compile_wf Phi U V G : forall  t b1 b2, 
+                                 IR.block_equiv U V Phi t G b1 b2 ->
+                                 forall G',
+                                   rel U V G G' ->                                  
+                                 block_equiv U V Phi t G' (compile Phi U t b1) (compile Phi V t b2). 
+  Proof. 
+    induction 1; simpl;  unfold IR.R, R in *. 
+    
+    - intros. inversion H0; t; simpl.
+      constructor; eauto. eapply compile_effects_wf; eauto. 
+      repeat rewrite foo. 
+      unfold R. 
+  
+    simpl. 
+    simpl. 
+    
+  inversion H. simpl. inversion H4;t; simpl.
+  
+  constructor; auto. 
+
+  revert H. Import Equality. dependent induction b. induction H.
+  
+  simpl. 
+ *)
+
+Arguments Evar {Phi Var t} v. 
+Arguments Eread {Phi Var t} v. 
+Arguments Eread_rf {Phi Var n t} _ _ . 
+Arguments Ebuiltin {Phi Var args res} _ _%dlist. 
+Arguments Econstant {Phi Var ty} _. 
+Arguments Emux {Phi Var t} _ _ _. 
+Arguments Efst {Phi Var l t} _. 
+Arguments Esnd {Phi Var l t} _. 
+Arguments Enth {Phi Var l t} _ _. 
+Arguments Etuple {Phi Var l} _%dlist. 
