src/IR.v
@@ -1,0 +1,961 @@
+Require Import Common. 
+Require Import Core.   
+Require Import Front. 
+  
+Section t. 
+  Variable Phi : state. 
+  Notation updates := (DList.T (option ∘ eval_sync) Phi). 
+  
+  Section defs. 
+  Variable R : type -> Type. 
+  (** Combinational bindings (expressions, register reads)  *)
+  Inductive bind (t : type) : Type := 
+  | bind_expr :  expr R t ->  bind t
+  | bind_reg_read : var Phi (Treg t) -> bind t
+  | bind_regfile_read : forall n, var Phi (Tregfile n t) -> R (Tint n) -> bind t. 
+    
+  Inductive telescope (A : Type): Type :=
+  | telescope_end : A -> telescope A
+  | telescope_bind : forall arg, bind arg -> (R arg -> telescope A) -> telescope A. 
+    
+  (* nested effects *)
+  Inductive neffect  : Type :=
+  | neffect_guard : forall (guard : expr R Tbool), list (neffect) -> neffect 
+  | neffect_reg_write : forall t, var Phi (Treg t) -> R t -> neffect
+  | neffect_regfile_write : forall n t, var Phi (Tregfile n t) -> R ( (Tint n)) -> R t -> neffect. 
+
+  Definition nblock t := telescope (R t * expr R Tbool * list neffect)%type. 
+  
+  Fixpoint compose {A B}
+                   (tA : telescope  A)
+                   (f : A -> telescope  B) :
+    telescope  B :=
+    match tA with
+      | telescope_end e => f e
+      | telescope_bind arg b cont => telescope_bind _  arg b (fun x => compose (cont x) f)
+    end.
+
+  Definition compose_block {t B} 
+                           (tA : nblock t)
+                           (f : R t -> expr R Tbool -> list neffect -> telescope B) :
+    telescope B :=
+    compose tA (fun x => match x with ((r,g),e) => f r g e end). 
+
+  Hint Unfold compose_block. 
+  Notation "x <- e1 ; e2" := (telescope_bind _ _ e1 (fun x => e2)) (right associativity, at level 80, e1 at next level).  
+  Notation " & e " := (telescope_end _ e) (at level 71). 
+  Notation "[< r , g , e >] :- t1 ; t2 " := (compose_block t1 (fun r g e => t2)) (right associativity, at level 80, t1 at next level). 
+  
+  Arguments neffect_guard guard%expr neffects%list. 
+  
+  (** * Compilation *)
+  (** This 'smart constructor' reduces the size of the guard, by using
+  the fact that [true] is a neutral element for [&&] *)
+  
+  Definition andb (a b : expr R Tbool): expr R Tbool :=
+    match a, b with 
+      | Econstant Tbool x, o 
+      | o, Econstant Tbool x => if x then o else (#b false)%expr
+      | _, _ => (a && b)%expr
+    end. 
+  
+
+  Definition orb (a b : expr R Tbool): expr R Tbool :=
+    match a, b with 
+      | Econstant Tbool x, o 
+      | o, Econstant Tbool x => if x then (#b true) else o
+      | _, _ => (a || b)%expr
+    end. 
+  
+  Definition convert  l : DList.T (expr R) l -> Tuple.of_list (expr R) l := 
+    DList.to_tuple (fun t X => X). 
+
+  (**  The compilation function itself *)  
+  Definition compile_inner (unit : R Tunit) t (a : action Phi R t) : telescope (R t * expr R Tbool * list neffect).  
+  refine (
+      let f := fix compile t (a : action Phi R t) : telescope (R t * expr R Tbool * list neffect):= 
+          match a with 
+            | Return t exp =>  
+                x <- (bind_expr _ exp); 
+                & (x, #b true, nil)
+            | Bind t u A F => 
+                [< rA, gA, eA >] :- compile _ A;
+                [< rB, gB, eB >] :- compile _ (F rA); 
+                & (rB, andb gA gB, List.app eA eB)             
+            | Assert exp => 
+                x <- (bind_expr _ exp); 
+                & (unit, !x, nil)%expr
+            | Primitive args res p exprs => _
+            | OrElse t A A' => 
+                [< rA, gA, eA >] :- compile _ A;
+                [< rA', gA', eA' >] :- compile _ A';
+                let e := neffect_guard gA eA in 
+                let e' := neffect_guard (andb (~ gA)  gA')%expr eA' in 
+                  r <- (bind_expr _ (Emux _ _ gA (!rA) (!rA'))%expr); 
+                  & ( r , (orb gA gA')%expr , [e;e'])%list
+          end in f t a).
+  (* primitive *)
+  revert exprs. 
+  refine (match p with
+            | register_read t v => _
+            | register_write t v => _
+            | regfile_read n t v  => _
+            | regfile_write n t v  => _
+          end); clear p; intros exprs. 
+  (* register read *)
+  refine (x <- (bind_reg_read _ v); &(x, #b true, nil)). 
+  (* register write *)
+  refine ( let env := convert _ exprs in 
+             let w := fst env in 
+               x <- bind_expr _ w; 
+           let e := ([neffect_reg_write _ v x])%list  in 
+             &( unit, #b true, e)
+         ). 
+  (* register file read *)
+  refine ( let env := convert _ exprs in 
+             let adr := fst env in 
+               adr <- bind_expr _ adr; 
+           x <- bind_regfile_read _ _ v adr; 
+           &( x, #b true, nil)
+         ). 
+  (* register file write *)
+  refine ( let env := convert _ exprs in 
+             match env with 
+               | (adr, (w, _)) => 
+                   adr <- bind_expr _ adr; 
+                   w <- bind_expr _ w;
+                   let e :=  ([neffect_regfile_write _ _ v  adr w])%list in                      
+                     &( unit, #b true, e)                      
+             end
+         ). 
+    (* or else *)  
+  Defined. 
+    
+    Definition compile t a :=   
+      (unit <- (bind_expr _ (# Ctt))%expr; compile_inner unit t a). 
+
+  
+  Inductive effect  : sync -> Type :=
+  | effect_reg_write : forall t,  R t -> R Tbool -> effect (Treg t)
+  | effect_regfile_write : forall n t,  R t -> R ( (Tint n)) -> R Tbool -> 
+                                                effect (Tregfile n t). 
+  
+  Definition effects := DList.T (option ∘ effect) Phi. 
+  
+  Definition init_effects : effects := @DList.init sync (option ∘ effect) (fun t : sync => None) Phi. 
+
+  Definition block t := telescope (R t * expr R Tbool *  effects). 
+    
+  Notation "e :-- t1 ; t2 " := (compose t1 (fun e => t2)) (right associativity, at level 80, e1 at next level).
+  Arguments Tuple.set {T F l t} _ _ _.  
+
+  Definition nblock_to_block {t} (B : nblock t) : block t. 
+  unfold block, nblock in *. 
+  
+  Definition inversion_effect_Treg t (e : effect (Treg t)) : (R t * R Tbool) :=
+    match e with 
+      | effect_reg_write _ x y => (x,y)
+    end. 
+
+  Definition inversion_effect_Tregfile t n (e: effect (Tregfile n t)): 
+    (R t * R ( (Tint n)) *R Tbool) :=
+    match e with 
+      | effect_regfile_write _ _ x y z => (x,y,z)
+    end. 
+
+  Definition merge s (a b : effect s) : telescope (effect s). 
+  refine (match s as s'  return effect s' -> effect s' -> telescope (effect s') with 
+              | Treg t => fun a b => 
+                           let (va,ga) := inversion_effect_Treg t a in 
+                           let (vb,gb) := inversion_effect_Treg t b in 
+                             (
+                               we <- bind_expr  _ (!ga || !gb)%expr ;
+                               w <- bind_expr  _ (Emux _ _ (!ga) (!va) (!vb) )%expr ;
+                               & (effect_reg_write  _ w we))
+              | Tregfile n t => fun a b => 
+                           match inversion_effect_Tregfile t n a with 
+                             | (va,adra,ga) =>
+                                 match inversion_effect_Tregfile t n b with 
+                                   | (vb,adrb,gb) =>
+                                       (
+                                         we <- bind_expr  _ (orb (!ga) (!gb))%expr; 
+                                         wadr <- bind_expr _ (Emux _ _ (!ga) (!adra) (!adrb))%expr; 
+                                         wdata <- bind_expr _ (Emux _ _ (!ga) (!va) (!vb))%expr; 
+                                         &  (effect_regfile_write _ _ wdata wadr we))
+                                 end
+                           end
+          end a b). 
+  Defined. 
+
+    (** We give the priority to the old write here  *)
+  Definition update t (v : var Phi t) (e : effect t)  (acc: effects) : telescope effects. 
+  refine ( match DList.get  v acc with 
+               | Some old => 
+                   e :-- merge t old e ; & (DList.set v (Some e) acc)
+               | None => 
+                   & (DList.set v (Some e) acc)
+           end). 
+  Defined. 
+                                                                       
+
+  Fixpoint compile_neffect (G : expr R Tbool) (E : neffect) (B : effects) : telescope effects :=
+    match E with               
+      | neffect_guard guard L => 
+                    let compile_neffects := fix compile_neffects G l U :=
+                        match l with 
+                          | nil =>  & U
+                          | cons t q => 
+                              compose (compile_neffect G t U)
+                                      (compile_neffects G q)
+                        end in 
+                      compile_neffects (andb G  guard)%expr L B
+      | neffect_reg_write t v val => 
+          G <- bind_expr _  G;
+          update (Treg t) v (effect_reg_write t val G) B
+      | neffect_regfile_write n t v adr val => 
+          G <- bind_expr _  G;
+          update (Tregfile n t) v (effect_regfile_write n t val adr G) B
+    end.  
+
+    
+  Fixpoint compile_neffects (G : expr R Tbool)(l : list neffect)  (T : effects) :
+    telescope effects :=
+    match l with 
+      | nil =>  & T
+      | cons t q => 
+          compose (compile_neffect G  t T)
+                  (compile_neffects G q)
+    end. 
+
+  (* guard was replaced by true  *)
+  refine (compose_block B (fun res guard neffects => 
+                             compose (compile_neffects (guard ) neffects (init_effects))
+                             (fun effects => &(res, guard, effects)))). 
+  Defined. 
+
+
+  End defs. 
+  
+  (** * Semantics *)
+  Section sem. 
+    Variable st : eval_state Phi. 
+    Definition eval_bind t (b : bind eval_type t) : (eval_type t).
+    refine (match b with
+              | bind_expr x =>  (eval_expr _ x)
+              | bind_reg_read v => (DList.get v st)
+              | bind_regfile_read n v adr => 
+                  let rf := DList.get  v st in
+                    Regfile.get rf (adr)                
+            end
+           ). 
+    Defined. 
+    
+                                                                
+    Fixpoint eval_neffect (e :neffect eval_type) (Delta : updates) : updates :=    
+      match e with 
+        | neffect_guard g l' => 
+            let fix eval_neffects l Delta := 
+                match l with 
+                  | nil => Delta
+                  | cons e q =>  
+                      let Delta := eval_neffect e Delta in 
+                        eval_neffects q Delta
+                end in     
+              match eval_expr _ g with 
+                | true => 
+                    eval_neffects l' Delta
+                | false => Delta
+            end
+      | neffect_reg_write t v w =>                                               
+          Front.Diff.add Phi Delta (Treg t) v w 
+      | neffect_regfile_write  n t v adr w  =>  
+          let rf := DList.get v st in                          
+            let rf := Regfile.set rf adr  w in 
+              Front.Diff.add Phi Delta (Tregfile n t) v rf            
+    end. 
+  
+    Fixpoint eval_neffects ( l : list (neffect eval_type)) Delta : updates :=
+      match l with 
+        | nil =>  Delta
+        | cons e q => (* do Delta <- eval_neffect e Delta;  *)
+            let Delta :=  (eval_neffect e Delta) in 
+            eval_neffects q Delta
+      end. 
+  
+    Lemma fold_eval_neffects :
+      (fix eval_neffects l Delta := 
+       match l with 
+                | nil =>  Delta
+                | cons e q => 
+                    let Delta := (eval_neffect e Delta) in 
+                      (* do Delta <- eval_neffect e Delta;  *)
+                      eval_neffects q Delta
+       end)= eval_neffects .
+    Proof. 
+      unfold eval_neffects. reflexivity.
+    Qed. 
+    
+    Fixpoint eval_nblock t  (T : nblock  eval_type t) :
+      updates -> option (eval_type t * updates) := 
+      match T with
+        | telescope_bind arg bind cont => 
+            fun Delta => 
+              let res := eval_bind _ bind in
+              eval_nblock _ (cont res) Delta
+        | telescope_end (p, g, e) => fun Delta =>
+                                      let g := eval_expr _ g  in             
+                                      if g then                                         
+                                        Some (p, eval_neffects e Delta)
+                                      else None
+    end. 
+    
+    
+    Arguments Tuple.set {T F l t} v _ _. 
+    Definition eval_effects (e : effects eval_type) (Delta : updates) : updates.  
+    unfold effects in e. 
+
+    (* refine (Tuple.fold Phi _ e Delta).  *)
+    refine (DList.map3 _ Phi e st Delta). 
+
+    Definition eval_effect (a : sync) :   
+      (option ∘ effect eval_type) a ->
+      eval_sync a -> (option ∘ eval_sync) a -> (option ∘ eval_sync) a. 
+    
+    refine (fun  eff => 
+              match eff with 
+                  | Some eff =>  
+                      match eff in effect _ s return eval_sync s -> (option ∘ eval_sync) s -> (option ∘ eval_sync) s  with 
+                        |  effect_reg_write t val we =>  fun _ old => 
+                             match old with 
+                               | Some _ => old
+                               | None => if we then Some val else None
+                             end
+                        |  effect_regfile_write n t val adr we => fun rf old =>
+                             match old with 
+                               | Some _ => old 
+                               | None => 
+                                   if we then 
+                                     let rf := Regfile.set rf adr val in 
+                                       Some rf
+                                   else 
+                                     None                                       
+                             end
+                      end
+                  | None => fun _ old => old            
+            end). 
+    Defined. 
+    apply eval_effect. 
+    Defined. 
+
+    Fixpoint eval_block t  (T : block eval_type t) :
+      updates -> option (eval_type t * updates) := 
+      match T with
+        | telescope_bind arg bind cont => 
+            fun Delta => 
+              let res := eval_bind _ bind in
+              eval_block _ (cont res) Delta
+        | telescope_end (p, g, e) => fun Delta =>
+                                      let g := eval_expr _ g  in             
+                                      if g then                                         
+                                        Some (p, eval_effects e Delta)
+                                      else None
+    end. 
+  
+     
+  End sem. 
+  
+  Section correctness. 
+  
+    
+    Notation C := (compile_inner eval_type tt). 
+    Lemma eval_andb_true x y : (eval_expr Tbool (andb eval_type x y)) = (eval_expr Tbool x && eval_expr Tbool y)%bool.
+    Proof. 
+      Import Equality Bool. 
+      
+      dependent destruction x; dependent destruction y; simpl;
+      repeat match goal with 
+                 c : constant B |- _ => destruct c
+               | x : eval_type Tbool |- _ => destruct x
+               | _ => idtac
+             end; rewrite ?andb_true_r, ?andb_true_l, ?andb_false_l , ?andb_false_r ; reflexivity.  
+    Qed. 
+
+    Lemma eval_orb_true x y : (eval_expr Tbool (orb eval_type x y)) = (eval_expr Tbool x || eval_expr Tbool y)%bool.
+    Proof. 
+      Import Equality Bool. 
+      
+      dependent destruction x; dependent destruction y; simpl;
+      repeat match goal with 
+                 c : constant B |- _ => destruct c
+               | x : eval_type Tbool |- _ => destruct x
+               | _ => idtac
+             end; rewrite ?orb_true_r, ?orb_true_l, ?orb_false_l , ?orb_false_r ; reflexivity.  
+    Qed. 
+
+
+    Lemma eval_neffects_append  st e f (Delta : updates) : 
+      eval_neffects st (e ++ f) Delta = 
+                   eval_neffects st f (eval_neffects st e Delta).              
+    Proof. 
+      revert Delta. 
+      induction e. 
+      + reflexivity. 
+      + intros Delta.
+        
+        simpl. rewrite IHe. reflexivity.  
+    Qed. 
+
+    Variable st : eval_state Phi. 
+
+    Notation "B / Delta " := (eval_nblock st _ B Delta). 
+    Theorem compile_correct t (a : action Phi eval_type t)  Delta:
+      eval_nblock st _ (C t a ) Delta =  (Front.Sem.eval_action a st Delta).
+    Proof. 
+      revert Delta. 
+      induction a. 
+      - intros.  reflexivity. 
+      - intros Delta. simpl. unfold  Sem.Dyn.Bind. rewrite <- IHa.
+        transitivity (
+            do ed <- (C t a) / Delta ; 
+            let (e,d) := ed in 
+              eval_nblock st u (C u (f e)) d
+                   ); 
+        [|destruct  ((C t a) / Delta) as [[ e d ]| ]; simpl; easy]. 
+        clear IHa H.
+        generalize (C t a) as T. intros T. clear a.
+        
+        induction T. destruct a as [[rA gA] eA]. 
+        simpl in *. 
+        case_eq (eval_expr Tbool gA); intros H.  simpl.
+        unfold compose_block; simpl compose.  
+        induction (C u (f rA)). simpl. destruct a as [[rB gB] eB]. simpl. 
+        * rewrite eval_neffects_append. rewrite eval_andb_true. rewrite H. simpl. reflexivity. 
+        * simpl. rewrite H0. reflexivity.         
+
+        * unfold compose_block. simpl. induction (C u (f rA)). destruct a as [[rB gB] eB]. simpl. 
+          rewrite eval_andb_true. rewrite H. reflexivity.  
+          simpl. rewrite H0. reflexivity. 
+        * unfold compose_block. simpl. unfold compose_block in H. rewrite H. reflexivity.
+
+      - simpl. intros. 
+          Ltac t :=
+            repeat match goal with 
+                     | |- context [check ?x ; ?y] => 
+                         let H := fresh "check" in 
+                           case_eq x; intros H
+                   end. 
+          t; trivial. 
+      -                         (* primitive *)
+      intros. destruct p.  
+        +  simpl. reflexivity. 
+        + simpl.
+              
+          set (x := DList.to_tuple eval_expr exprs). 
+          replace (x) with (fst x, snd x) by (destruct x; reflexivity).
+          simpl.
+          DList.inversion. simpl. reflexivity. 
+
+        + simpl. 
+          DList.inversion; reflexivity.
+        + simpl. repeat DList.inversion. simpl. reflexivity.
+          Arguments andb R _ _ : simpl never. 
+          Arguments orb R _ _ : simpl never. 
+          Ltac s :=
+            match goal with 
+              |- context [eval_expr _ (orb _ ?x ?y )] => rewrite eval_orb_true
+            | |- context [eval_expr _ (andb _ ?x ?y )] => rewrite eval_andb_true
+            | H : context [eval_expr _ (orb _ ?x ?y )] |- _ => rewrite eval_orb_true in H
+            | H : context [eval_expr _ (andb _ ?x ?y )] |- _  => rewrite eval_andb_true in H
+            | H : eval_expr _ ?x = true |- context [eval_expr _ ?x] => rewrite H
+            | H : eval_expr _ ?x = true , H' : context [eval_expr _ ?x] |- _ => rewrite H in H'
+            | H : eval_expr _ ?x = false |- context [eval_expr _ ?x] => rewrite H
+            | H : eval_expr _ ?x = false , H' : context [eval_expr _ ?x] |- _ => rewrite H in H'
+            end. 
+      - intros. simpl.   unfold Sem.Dyn.OrElse. 
+        rewrite <- IHa1, <- IHa2 . clear IHa1 IHa2. 
+        generalize (C t a1); intros T; generalize (C t a2); intros T'. 
+        induction T as [[[rA gA] eA] |]; simpl.
+        induction T' as [[[rA' gA'] eA'] |]. simpl compose.
+        t. simpl. repeat (s; simpl). reflexivity. 
+        t. simpl. repeat (s; simpl). t. reflexivity. 
+        reflexivity. 
+        simpl. unfold compose_block in *. simpl in *.  rewrite H. reflexivity. 
+        simpl. unfold compose_block in *. simpl in *.  rewrite H. reflexivity. 
+
+    Qed.
+     
+  End correctness.     
+ End t. 
+
+Section correctness2. 
+  
+  Notation Cs  := (compile_neffects  _ _).
+  Notation C  := (compile_neffect  _ _).
+  Notation "x <- e1 ; e2" := (@telescope_bind _ _ _ _ _ e1 (fun x => e2)) (right associativity, at level 80, e1 at next level).
+  Notation " & e " := (@telescope_end _ _ _ e) (at level 71).
+  Notation "e :- t1 ; t2 " := (@compose  _ _ _ _ t1 (fun e => t2)) (right associativity, at level 80, t1 at next level).
+
+  
+
+  Ltac t := simpl; intuition; try match goal with
+                                    | [ H : _ |- _ ] => rewrite H; auto
+                                end.
+   
+  
+  Lemma eval_effect_init Phi st Delta : eval_effects Phi st (init_effects Phi eval_type) Delta = Delta. 
+  Proof.
+    unfold eval_effects. 
+    induction Phi. simpl. reflexivity. 
+    simpl. repeat DList.inversion. simpl. f_equal. apply IHPhi. 
+  Qed. 
+
+  Lemma foo {Phi R A B C} (T: telescope Phi R A) (f : A -> telescope  Phi R B)  (g : B -> telescope Phi R C) :
+    (X :- (Y :- T; f Y); (g X) )= (Y :- T; X :- f Y; g X).
+  Proof.
+      induction T. reflexivity. simpl.
+      f_equal.
+      Require Import  FunctionalExtensionality.
+      apply functional_extensionality.
+      apply H.
+  Qed.
+     
+  Lemma my_ind Phi (R : type -> Type) (P : neffect Phi R -> Prop) :
+    (forall (guard : expr R Tbool) ,
+       P (neffect_guard Phi  R guard [])) ->
+    (forall (guard : expr R Tbool) a l ,
+       P a -> P (neffect_guard Phi  R guard l) ->
+       P (neffect_guard Phi  R guard (a :: l))) ->
+    (forall (t : type) (v : var Phi (Treg t)) (r : R t),
+       P (neffect_reg_write  Phi R t v r)) ->
+    (forall (n : nat) (t : type) (v : var Phi (Tregfile n t))
+       (r : R ( (Tint n))) (r0 : R t),
+       P (neffect_regfile_write Phi R n t v r r0)) ->
+    forall n : neffect Phi R, P n. 
+  Proof.
+    intros. 
+    refine (let fold := fix fold n :=
+        match n with
+            | neffect_guard g l => 
+                let fix foldi l : P (neffect_guard Phi R g l) :=
+                    match l return  P (neffect_guard Phi R g l) with 
+                      | nil => H g
+                      | cons t q => H0 g t q (fold t) (foldi q)
+                    end in foldi l
+            | neffect_reg_write t v w => H1 t v w
+            | neffect_regfile_write n t v adr w => H2 n t v adr w
+        end in fold n). 
+  Qed. 
+  
+  Lemma correspondance Phi l e : forall g1 g2, 
+                               compile_neffect Phi eval_type g1 (neffect_guard Phi eval_type g2 l) e = (compile_neffects Phi eval_type (andb _ g1  g2)%expr l e).
+  Proof.                                                                                        
+    induction l; reflexivity.
+  Qed. 
+  
+  Lemma eval_neffect_cons Phi st guard a l Delta: 
+    eval_neffect Phi st (neffect_guard Phi eval_type guard (a :: l)) Delta = 
+                 (if eval_expr Tbool guard
+                  then eval_neffects Phi st l (eval_neffect Phi st a Delta)
+                  else Delta).
+  Proof. 
+    reflexivity. 
+  Qed.
+  
+  Fixpoint eval_telescope { A B} Phi st (F : A -> B) (T : telescope  Phi eval_type A) :=
+    match T with 
+      | telescope_end X => F X
+      | telescope_bind arg bind cont =>
+          let res := eval_bind Phi st arg bind in 
+            eval_telescope Phi st F (cont res)
+    end. 
+
+  Lemma folder Phi st guard l Delta: eval_neffect Phi st (neffect_guard  Phi eval_type guard l) Delta 
+                                         = if eval_expr Tbool guard then eval_neffects Phi st l Delta else Delta.
+  Proof. 
+    reflexivity. 
+  Qed. 
+    
+
+  
+  Notation "[[ x ]]" := (eval_expr Tbool x). 
+  Arguments Tuple.set {T F l t} _ _ _.
+  Arguments Tuple.get {T F l t} _ _. 
+
+  Notation Ev Phi st  := (eval_telescope Phi st (eval_effects Phi st)).  
+  
+  Ltac v := match goal with 
+                |- context [match ?X with  | ( _ , _  )  => _ end ] => destruct X 
+            end. 
+  Import Equality. 
+  Ltac d := match goal with 
+              | H : context [match ?X with | _ => _ end] |- _ => dependent destruction X
+              |  |- context [match ?X with | _ => _ end] => case_eq  X; intros; subst; simpl
+                                                                                      
+            end. 
+
+  Lemma rew_1 Phi st Delta t (v : var Phi t ) x e : 
+    eval_effects Phi st (DList.set v (Some x) e) Delta =
+                 DList.set v (eval_effect t (Some x) (DList.get v st) (DList.get v Delta))  (eval_effects Phi st e Delta).  
+  Proof. 
+    induction Phi; [dependent destruction v|]. 
+    dependent destruction v. 
+    simpl; repeat v; destruct x; simpl; d; f_equal.
+    simpl. repeat v; destruct x; simpl; rewrite IHPhi; clear IHPhi; 
+           simpl; repeat d; simpl in *; auto. 
+  Qed. 
+
+  Lemma inversion_1 Phi st : forall t (v : var Phi (Treg t)) e Delta x x', 
+                             inversion_effect_Treg eval_type t x = (x', true) ->
+                             DList.get v e = Some x ->
+                             exists y, DList.get v (eval_effects Phi st e Delta) = Some y.
+  Proof. 
+    induction Phi; [dependent destruction v|]. 
+    dependent destruction v; simpl; intros. 
+    repeat v; dependent destruction x; simpl in *; inversion H; subst; clear H; simpl.
+    repeat DList.inversion.  simpl in H0. subst. simpl.
+    d; eauto.
+
+    simpl in *. repeat v. simpl. edestruct IHPhi; eauto.
+  Qed. 
+
+
+  Lemma compile_effect_correct Phi st a  : 
+    forall Delta e g , 
+      eval_telescope Phi st (eval_effects Phi st) (C g a e) Delta 
+                     =  if [[g]] then eval_neffect Phi st a (Ev Phi st (&e) Delta) else (Ev Phi st (&e)Delta). 
+  Proof. 
+      induction a using my_ind. 
+      - intros. simpl. destruct ([[guard]]); destruct ([[g]]); reflexivity.
+      - intros. rewrite correspondance. rewrite eval_neffect_cons. 
+        simpl compile_neffects. simpl.
+        setoid_rewrite correspondance in IHa0.
+        
+        revert IHa IHa0.
+        intros H. specialize (H Delta e (andb _ g guard)%expr). revert H. 
+        induction (C (andb _ g guard)%expr a e); intros. 
+        {simpl. rewrite IHa0. rewrite folder. simpl. simpl in H. rewrite eval_andb_true in H.        simpl in H. 
+         destruct ([[g]]); destruct ([[guard]]); simpl; simpl in H; try rewrite H; try reflexivity. }
+         {
+         simpl. rewrite H. reflexivity. 
+         simpl. simpl in *. rewrite H0. reflexivity.
+         apply IHa0.          
+         }
+      - intros. simpl.
+        unfold update. 
+        case_eq (DList.get  v e); intros; simpl. 
+        +               
+        (* case: there was a previous effect on this register *)
+        case_eq (inversion_effect_Treg eval_type t e0); intros; simpl.       
+          
+        
+        rewrite rew_1. 
+        case_eq (e2); intros; simpl. 
+          * destruct ([[g]]). 
+            subst. 
+            {
+              Lemma hint_1 Phi : forall st t (v : var Phi (Treg t)) r Delta e  e0, 
+                                 DList.get v e = Some e0 -> 
+                                 forall e1, inversion_effect_Treg eval_type t e0 = (e1, true) -> 
+                                       DList.set v
+                                            match DList.get v Delta with
+                                                | Some _ => DList.get v Delta
+                                                | None => Some e1
+              end (eval_effects Phi st e Delta) =
+                                          Diff.add Phi (eval_effects Phi st e Delta) (Treg t) v r. 
+              Proof. 
+                
+                induction Phi; [dependent destruction v|].
+                simpl. intros; repeat v. 
+                 dependent destruction v; simpl; intros. 
+                 repeat DList.inversion.  
+                 unfold Diff.add;  simpl; repeat d; simpl in *; subst;
+                 simpl in H1; dependent destruction e0; f_equal; auto.
+                 discriminate. 
+                 simpl in *; inversion H0; subst; auto. 
+                 simpl in *; inversion H0; subst; discriminate.
+                 simpl in *. setoid_rewrite IHPhi. unfold Diff.add.  simpl.
+                 repeat d; reflexivity.
+                 eauto. 
+                 eauto. 
+              Qed.
+            eapply hint_1; eauto. 
+            }
+            subst.
+            {
+              induction Phi; [dependent destruction v|]. 
+              simpl; repeat v. 
+              dependent destruction v; simpl in *; subst. unfold Diff.add.
+               unfold effects in *.  repeat DList.inversion. simpl in *.
+              repeat d; clear IHPhi; dependent destruction e0;subst; f_equal; auto. 
+              simpl in H0. inversion H0; subst. auto.
+              simpl. rewrite IHPhi. auto. auto. 
+            }
+         
+            
+
+          * subst.
+            destruct ([[g]]). 
+            simpl. 
+            unfold Diff.add. 
+            {
+            induction Phi; [dependent destruction v|]. 
+              simpl; repeat v. 
+              dependent destruction v; simpl in *; subst. unfold Diff.add.
+               unfold effects in *.  repeat DList.inversion. simpl in *.
+
+              repeat d; clear IHPhi; dependent destruction e0;subst; f_equal; auto. 
+              discriminate. simpl in *; inversion H0; subst; auto. 
+              simpl in *; inversion H0; subst; auto. 
+              discriminate.
+              
+              setoid_rewrite IHPhi. clear IHPhi. unfold Diff.add. simpl. d. reflexivity.
+              reflexivity. 
+              auto. 
+            }
+            
+            {
+            induction Phi; [dependent destruction v|]. 
+              simpl; repeat v. 
+              dependent destruction v; simpl in *; subst. unfold Diff.add.
+               unfold effects in *.  repeat DList.inversion. simpl in *.
+
+              repeat d; clear IHPhi; dependent destruction e0;subst; f_equal; auto. 
+              simpl in *. inversion H0; auto. 
+              
+              setoid_rewrite IHPhi. auto.  auto. 
+            
+            }
+            
+            
+            
+        + rewrite rew_1. simpl. 
+
+          unfold Diff.add. 
+          {
+          
+            induction Phi; [dependent destruction v|]. 
+              simpl; repeat v. 
+              dependent destruction v; simpl in *; subst. unfold Diff.add.
+               unfold effects in *.  repeat DList.inversion. simpl in *.
+repeat d; repeat f_equal. 
+              
+              setoid_rewrite IHPhi. clear IHPhi. unfold Diff.add. simpl. repeat d; f_equal. auto. 
+          }
+
+      - intros. simpl.         unfold update. 
+        case_eq (DList.get v e); intros; simpl. 
+        +               
+        case_eq (inversion_effect_Tregfile eval_type t n e0); intros [w adr we H']; simpl.         
+        rewrite rew_1.
+        simpl.
+        case_eq (we); intros; simpl. 
+        * destruct [[g]]. 
+          unfold Diff.add.
+          {
+            induction Phi; [dependent destruction v|].
+            simpl; repeat v. 
+            dependent destruction v; simpl in *; subst.
+             unfold effects in *.  repeat DList.inversion. simpl in *; subst. 
+            
+
+            unfold Diff.add; repeat d; repeat f_equal; dependent destruction e0; simpl in H'; inversion H'; subst;  try congruence; try simpl in *; try auto.
+            rewrite IHPhi; clear IHPhi;  auto. 
+            unfold Diff.add; repeat d; repeat f_equal; dependent destruction e0; simpl in H'; inversion H'; subst;  try congruence; try simpl in *; try auto.
+          }
+          subst. 
+          {
+            induction Phi; [dependent destruction v|].
+            simpl; repeat v. 
+            dependent destruction v; simpl in *; subst. 
+             unfold effects in *.  repeat DList.inversion. simpl in *; subst. 
+
+            unfold Diff.add; repeat d; repeat f_equal; dependent destruction e0; simpl in H'; inversion H'; subst;  try congruence; try simpl in *; try auto.
+            rewrite IHPhi; clear IHPhi;  auto. 
+          }
+
+          *destruct [[g]]. subst. 
+          unfold Diff.add. 
+          {
+              induction Phi; [dependent destruction v|].
+            simpl; repeat v. 
+            dependent destruction v; simpl in *; subst. 
+                         unfold effects in *.  repeat DList.inversion. simpl in *; subst. 
+unfold Diff.add; repeat d; repeat f_equal; dependent destruction e0; simpl in H'; inversion H'; subst;  try congruence; try simpl in *; try auto.
+            rewrite IHPhi; clear IHPhi;  auto. 
+            repeat d; repeat f_equal; dependent destruction e0; simpl in H'; inversion H'; subst;  try congruence; try simpl in *; try auto.          
+          }
+          {
+            induction Phi; [dependent destruction v|].
+            simpl; repeat v. 
+            dependent destruction v; simpl in *; subst. unfold Diff.add.
+                         unfold effects in *.  repeat DList.inversion. simpl in *; subst. 
+repeat d; repeat f_equal; dependent destruction e0; simpl in H'; inversion H'; subst;  try congruence; try simpl in *; try auto.
+            rewrite IHPhi; clear IHPhi; auto. }
+          
+          
+        + rewrite rew_1. simpl.
+          unfold Diff.add. 
+          {
+            induction Phi; [dependent destruction v|].
+            simpl; repeat v. 
+            dependent destruction v; simpl in *; subst. unfold Diff.add.
+             unfold effects in *.  repeat DList.inversion. simpl in *; subst. 
+
+            repeat d; repeat f_equal; dependent destruction e0; simpl in H'; inversion H'; subst;  try congruence; try simpl in *; try auto.
+            rewrite IHPhi; clear IHPhi; auto. 
+            repeat d; repeat f_equal; dependent destruction e0; simpl in H'; inversion H'; subst;  try congruence; try simpl in *; try auto. 
+
+          }
+    Qed. 
+
+    Lemma eval_telescope_neffects Phi st es : forall Delta e g, eval_telescope Phi st (eval_effects Phi st) (Cs g es e) Delta 
+                               =  if [[g]] then eval_neffects Phi st es (Ev Phi st (&e) Delta) else Ev Phi st (&e) Delta. 
+    Proof. 
+      induction es. 
+      intros; simpl.  destruct ([[g]]); reflexivity.  
+      simpl. intros. 
+      pose (H := compile_effect_correct Phi st a Delta e g). 
+      clearbody H. revert H. 
+      induction (C g a e). 
+      - simpl.       intros H. 
+      rewrite IHes. simpl. rewrite H. destruct ([[g]]); reflexivity.
+      - simpl. intros. apply H. simpl. auto.  
+    Qed. 
+ 
+    Theorem nblock_compile_correct Phi (st : eval_state Phi) t (nb : nblock Phi eval_type t)  Delta:
+      eval_block Phi st _  (nblock_to_block Phi eval_type nb) Delta =  eval_nblock Phi st _ nb Delta. 
+      unfold nblock in nb. 
+      induction nb as [ [ [rA gA] eA]|]. 
+      2: simpl; rewrite <- H; reflexivity. 
+      
+      {
+        unfold nblock_to_block. unfold compose_block. simpl.
+        pose (H := eval_telescope_neffects Phi st eA Delta (init_effects Phi eval_type) gA). 
+        clearbody H. 
+        case_eq ([[gA]]).
+        {
+          intros. rewrite H0 in H. simpl in H. 
+          rewrite eval_effect_init in H. 
+          rewrite <- H. clear H.  
+          induction (Cs gA eA (init_effects Phi eval_type)). simpl. rewrite H0. reflexivity. 
+          simpl. rewrite <- H. reflexivity. 
+        }
+        {
+          intros.
+          induction (Cs gA eA (init_effects Phi eval_type)). simpl. rewrite H0. reflexivity. 
+          simpl. apply H1. auto.          
+        }
+      }
+
+    Qed. 
+  
+End correctness2. 
+
+Definition Block Phi t := forall V,  block Phi V t. 
+Definition Compile Phi t (A : forall V, action Phi V t) : Block Phi t := 
+  fun V =>
+    nblock_to_block Phi V (compile Phi V t (A V)):block Phi V t. 
+Definition Eval Phi st t (B : Block Phi t) Delta :=
+  eval_block Phi st t (B _) Delta. 
+
+
+Theorem Compile_correct Phi t A : forall st Delta,
+  Eval Phi st t (Compile Phi t A) Delta =  Front.Eval Phi st t A Delta. 
+Proof. 
+  unfold Compile, Eval, Front.Eval. intros. 
+  rewrite nblock_compile_correct. 
+  simpl.  rewrite compile_correct. reflexivity.   
+Qed. 
+
+
+Section equiv. 
+  Import Core. 
+  Variable U V : type -> Type. 
+  Variable Phi : state. 
+
+  Reserved Notation "x == y" (at level 70, no associativity). 
+  Reserved Notation "x ==e y" (at level 70, no associativity). 
+  
+  Section inner_equiv. 
+  Variable R : forall t, U t -> V t -> Prop. 
+  Notation "x -- y" := (R _ x y) (at level 70, no associativity). 
+    
+  Inductive expr_equiv : forall t,  expr U t -> expr  V t -> Prop :=
+  | Eq_var : forall  t (v1 : U t) v2, v1 -- v2 -> Evar v1 == Evar v2
+  | Eq_builtin : forall args res (f : builtin args res) dl1 dl2, 
+                   Common.DList.pointwise expr_equiv args dl1 dl2 ->
+                   Ebuiltin  f dl1 == Ebuiltin  f dl2
+  | Eq_constant : forall ty (c : constant ty), Econstant c == Econstant c
+  | Eq_mux : forall t c1 c2 l1 l2 r1 r2, 
+               c1 == c2 -> l1 == l2 -> r1 == r2 -> 
+               Emux  U t c1 l1 r1 ==  Emux  V t c2 l2 r2
+                    
+  | Eq_fst : forall (l : list type) (t : type) dl1 dl2, 
+               dl1 == dl2 -> 
+               Efst  U l t dl1 == Efst  V l t dl2
+
+  | Eq_snd : forall (l : list type) (t : type) dl1 dl2, 
+               dl1 == dl2 -> 
+               Esnd  U l t dl1 == Esnd  V l t dl2
+
+  | Eq_nth : forall (l : list type) (t : type) (v : Common.var l t)  dl1 dl2, 
+               dl1 == dl2 -> 
+               Enth v dl1 == Enth v dl2
+
+  | Eq_tuple : forall (l : list type) dl1 dl2, 
+                 Common.DList.pointwise expr_equiv l dl1 dl2 ->
+               Etuple  U l dl1 == Etuple  V l dl2
+                            where "x == y" := (expr_equiv _ x y). 
+  
+  Inductive effect_equiv : forall t,  option (effect U t) -> option (effect V t) -> Prop :=
+  | Eq_none : forall t, effect_equiv t None None
+  | Eq_write : forall t v1 v2 we1 we2, 
+                 v1 -- v2 -> we1 -- we2 -> 
+                 Some (effect_reg_write U t v1 we1) ==e Some  (effect_reg_write V t v2 we2)
+  | Eq_write_rf : forall n t v1 v2 adr1 adr2 we1 we2, 
+                    v1 -- v2 -> adr1 -- adr2 -> we1 -- we2 -> 
+                    Some (effect_regfile_write U n t v1 adr1 we1) ==e 
+                         Some (effect_regfile_write V n t v2 adr2 we2)
+                                  where "x ==e y" := (effect_equiv _ x y). 
+ 
+  Definition effects_equiv : effects Phi U -> effects Phi V -> Prop := 
+    Common.DList.pointwise  effect_equiv Phi. 
+  
+  End inner_equiv. 
+ 
+  Inductive Gamma : Type :=
+  | nil : Gamma
+  | cons : forall t, U t -> V t -> Gamma -> Gamma. 
+  
+  Inductive In t (x : U t) (y : V t) : Gamma -> Prop :=
+  | In_ok : forall Gamma x' y', x' = x -> y' = y ->
+              In t x y (cons t x' y' Gamma )
+  | In_skip : forall Gamma t' x' y', 
+                In t x y Gamma -> 
+                In t x y (cons t' x' y' Gamma ). 
+
+  Definition R G := fun t x y => In t x y G.  
+
+  Reserved Notation "G |- x ==b y" (at level 70, no associativity). 
+  Notation "G |- x -- y" := (In _ x y G) (at level 70, no associativity). 
+
+  Inductive bind_equiv t : forall (G : Gamma), bind Phi U t -> bind Phi V t -> Prop :=
+  |Eq_expr : forall G v1 v2, expr_equiv (R G) t v1 v2 ->
+                        bind_equiv t G (bind_expr Phi U t v1) (bind_expr Phi V t v2)
+  |Eq_reg : forall G v, bind_equiv t G  (bind_reg_read Phi U t v) (bind_reg_read Phi V t v)
+  |Eq_regfile : forall G n v a1 a2, 
+                  G |- a1 -- a2 ->
+                  bind_equiv t G  (bind_regfile_read Phi U t n v a1) (bind_regfile_read Phi V t n v a2). 
+
+  Inductive block_equiv t : forall (G : Gamma), block Phi U t -> block Phi V t -> Prop :=
+  | Eq_end : forall G (v1 : U t) v2 g1 g2 e1 e2, 
+               G |- v1 -- v2 ->  expr_equiv (R G) _ g1 g2 -> effects_equiv (R G) e1 e2 ->
+               G |- telescope_end Phi U _ (v1, g1, e1) ==b telescope_end Phi V _ (v2,g2, e2 ) 
+  | Eq_bind : forall G a (e1 : bind Phi U a) e2 (k1 : U a -> block Phi U t) k2,
+                bind_equiv _ G e1 e2 -> 
+                (forall v1 v2, (* G |- v1 -- v2 ->  *)cons _ v1 v2 G |- k1 v1 ==b k2 v2) ->
+                G |- telescope_bind Phi U _ a e1 k1 ==b telescope_bind Phi V _ a e2 k2                
+                 where "G |- x ==b y" := (block_equiv _ G x y). 
+End equiv. 
+
+Definition WF Phi t (b : Block Phi t) := forall U V, block_equiv U V Phi t (nil _ _) (b _) (b _). 
