talks/coq-2012/phoas.v
@@ -1,0 +1,18 @@
+Inductive T : Type :=
+  | Tbool
+  | Tarrow : T -> T -> T. 
+
+Section t. 
+
+  Variable V : T -> Type. 
+  Inductive term : T -> Type :=
+  | Var : forall t, V t -> term t
+  | Abs : forall a b, (V a -> term b) -> term (Tarrow a b)
+  | App : forall a b, term (Tarrow a b) -> term a -> term b. 
+End t.  
+
+Definition Term t := forall V, term V t. 
+
+Arguments Abs {V a b} _. 
+Arguments Var {V t} _. 
+Example K a b : Term (Tarrow a (Tarrow b a))  := fun V => Abs (fun x => Abs (fun y => Var x)). 
